format-version: 1.0
date: 10:06:2006 18:12
saved-by: whetzel
auto-generated-by: OBO-Edit 1.000
default-namespace: PSI-MS

[Term]
id: PSI:0000000
name: mzOntology

[Term]
id: PSI:1000001
name: Sample Number
def: "A reference number relevant to the sample under study." [PSI:GPS]
relationship: part_of PSI:1000457 ! Sample Description

[Term]
id: PSI:1000002
name: Sample Name
def: "A reference string relevant to the sample under study." [PSI:GPS]
relationship: part_of PSI:1000457 ! Sample Description

[Term]
id: PSI:1000003
name: Sample State
def: "The chemical phase of a pure sample, or the state of a mixed sample." [PSI:GPS]
relationship: part_of PSI:1000457 ! Sample Description

[Term]
id: PSI:1000004
name: Sample Mass
def: "Total mass of sample used in generating this individual mzData file." [PSI:GPS]
relationship: part_of PSI:1000457 ! Sample Description

[Term]
id: PSI:1000005
name: Sample Volume
def: "Total volume of solution used in generating this individual mzData file." [PSI:GPS]
relationship: part_of PSI:1000457 ! Sample Description

[Term]
id: PSI:1000006
name: Sample Concentration
def: "Concentration of sample in solution used in generating this individual mzData file." [PSI:GPS]
relationship: part_of PSI:1000457 ! Sample Description

[Term]
id: PSI:1000007
name: Inlet Type
def: "The nature of the sample inlet" [PSI:GPS]
relationship: part_of PSI:1000458 ! Source Description

[Term]
id: PSI:1000008
name: Ionization Type
def: "The method by which ions are generated from the sample" [PSI:GPS]
relationship: part_of PSI:1000458 ! Source Description

[Term]
id: PSI:1000009
name: Ionization Mode
def: "Whether positive or negative ions are selected for analysis by the spectrometer. Re-map to Polarity Mode." [PSI:GPS]
is_obsolete: true

[Term]
id: PSI:1000010
name: Analyzer Type
def: "The common name of the particular analyzer stage being described" [PSI:GPS]
relationship: part_of PSI:1000451 ! Analyzer Description

[Term]
id: PSI:1000011
name: Mass Resolution
def: "The maximum m/z value at which two peaks can be resolved, according to one of the standard measures." [PSI:GPS]
is_a: PSI:1000444 ! m/z Separation Method

[Term]
id: PSI:1000012
name: Resolution Method
def: "Which of the available standard measures is used to define whether two peaks are separate" [PSI:GPS]
relationship: part_of PSI:1000451 ! Analyzer Description

[Term]
id: PSI:1000013
name: Resolution Type
def: "Specify the nature of resolution for the mass analyzer.  Resolution is usually either constant with respect to m/z or proportional to m/z." [PSI:GPS]
relationship: part_of PSI:1000451 ! Analyzer Description

[Term]
id: PSI:1000014
name: Accuracy
def: "Accuracy of mass assignment" [PSI:GPS]
relationship: part_of PSI:1000451 ! Analyzer Description

[Term]
id: PSI:1000015
name: Scan Rate
def: "Rate in (m/z)/sec for scanning analyzers" [PSI:GPS]
relationship: part_of PSI:1000451 ! Analyzer Description

[Term]
id: PSI:1000016
name: Scan Time
def: "Time taken for an acquisition for scanning analyzers" [PSI:GPS]
relationship: part_of PSI:1000451 ! Analyzer Description

[Term]
id: PSI:1000017
name: Scan Function
def: "Describes the type of mass analysis being performed.  Two primary modes are typical: acquisition over a range of masses (MassScan), and SelectionIonDetection.  The primary difference is that Selected Ion Detection produces a single value for the signal at the selected mass rather than producing a mass spectrum. " [PSI:GPS]
relationship: part_of PSI:1000451 ! Analyzer Description

[Term]
id: PSI:1000018
name: Scan Direction
def: "Direction in terms of m/z of the scan for scanning analyzers (low to high, or high to low)." [PSI:GPS]
relationship: part_of PSI:1000451 ! Analyzer Description

[Term]
id: PSI:1000019
name: Scan Law
def: "Describes the function in control of the m/z scan (for scanning instruments).  Commonly the scan function is linear, but in principle any function can be used." [PSI:GPS]
relationship: part_of PSI:1000451 ! Analyzer Description

[Term]
id: PSI:1000020
name: Tandem Scanning Method
def: "Describes the acquisition data type produced by a tandem mass spectrometry experiment.  " [PSI:GPS]
relationship: part_of PSI:1000451 ! Analyzer Description

[Term]
id: PSI:1000021
name: Reflectron State
def: "Status of the reflectron, turned on, off or no reflectron." [PSI:GPS]
relationship: part_of PSI:1000451 ! Analyzer Description

[Term]
id: PSI:1000022
name: TOF Total Path Length
def: "The length of the field free drift space in a time of flight mass spectrometer." [PSI:GPS]
relationship: part_of PSI:1000451 ! Analyzer Description

[Term]
id: PSI:1000023
name: Isolation Width
def: "The total width (i.e. not half for plus-or-minus) of the gate applied around a selected precursor ion." [PSI:GPS]
relationship: part_of PSI:1000451 ! Analyzer Description

[Term]
id: PSI:1000024
name: Final MS Exponent
def: "The final MS level achieved when performing PFF with the ion trap (e.g. MS E10)." [PSI:GPS]
relationship: part_of PSI:1000451 ! Analyzer Description

[Term]
id: PSI:1000025
name: Magnetic Field Strength
def: "A property of space that produces a force on a charged particle equal to qv x B where q is the particle charge and v its velocity." [PSI:GPS]
related_synonym: "Magnetic Field" []
exact_synonym: "B" []
relationship: part_of PSI:1000451 ! Analyzer Description

[Term]
id: PSI:1000026
name: Detector Type
def: "The type of the detector used to detect the ions in the mass spectrometer." [PSI:GPS]
relationship: part_of PSI:1000453 ! Detector Description

[Term]
id: PSI:1000027
name: Detector Acquisition Mode
def: "Method by which detector signal is acquired by the data system." [PSI:GPS]
relationship: part_of PSI:1000453 ! Detector Description

[Term]
id: PSI:1000028
name: Detector Resolution
def: "The resolving power of the detector to differentiate between ions of two different m/z values." [PSI:GPS]
relationship: part_of PSI:1000453 ! Detector Description

[Term]
id: PSI:1000029
name: Sampling Frequency
def: "The rate of signal sampling (measurement) with respect to time." [PSI:GPS]
narrow_synonym: "ADC Sampling Frequency" []
relationship: part_of PSI:1000453 ! Detector Description

[Term]
id: PSI:1000030
name: Vendor
def: "Name of instrument vendor" [PSI:GPS]
relationship: part_of PSI:1000454 ! Instrument Additional Description

[Term]
id: PSI:1000031
name: Model
def: "Instrument's model name (everything but the vendor's name)" [PSI:GPS]
relationship: part_of PSI:1000454 ! Instrument Additional Description

[Term]
id: PSI:1000032
name: Customization
def: "Free text description of a single customization made to the instrument; for several modifications, use several entries" [PSI:GPS]
relationship: part_of PSI:1000454 ! Instrument Additional Description

[Term]
id: PSI:1000033
name: Deisotoping
def: "Deisotoping is removal of isotopes to represent the fragment ion as one data point and is commonly done to reduce complexity. It is done in conjunction with the charge state deconvolution." [PSI:GPS]
relationship: part_of PSI:1000452 ! Data Processing Method

[Term]
id: PSI:1000034
name: Charge Deconvolution
def: "The determination of the mass of an ion based on the mass spectral peaks that represent multiple-charge ions." [PSI:GPS]
relationship: part_of PSI:1000452 ! Data Processing Method

[Term]
id: PSI:1000035
name: Peak Processing
def: "Spectral peak processing done on the acquired data." [PSI:GPS]
relationship: part_of PSI:1000452 ! Data Processing Method

[Term]
id: PSI:1000036
name: Scan Mode
def: "TODO: Add definition." [PSI:GPS]
#is_obsolete: true THIS TERM SHOULD NOT BE OBSOLETE, BECAUSE THERE IS NO REPLACEMENT...

[Term]
id: PSI:1000037
name: Polarity
def: "Terms to describe the polarity setting of the instrument." [PSI:GPS]
relationship: part_of PSI:1000459 ! Spectrum Instrument Description

[Term]
id: PSI:1000038
name: Time In Minutes
def: "Acquisition time in minutes." [PSI:GPS]
is_a: PSI:1000460 ! Unit
relationship: part_of PSI:1000459 ! Spectrum Instrument Description

[Term]
id: PSI:1000039
name: Time In Seconds
def: "Acquisition time in seconds." [PSI:GPS]
is_a: PSI:1000460 ! Unit
relationship: part_of PSI:1000459 ! Spectrum Instrument Description

[Term]
id: PSI:1000040
name: Mass To Charge Ratio
def: "The symbol m/z is used to denote the dimensionless quantity formed by dividing the mass of an ion in atomic units by its charge number. The symbol is italicized lower case letters with no spaces." [PSI:GPS]
exact_synonym: "m/z" []
relationship: part_of PSI:1000455 ! Ion Selection Description

[Term]
id: PSI:1000041
name: Charge State
def: "The charge state of the ion, single or multiple and positive or negatively charged." [PSI:GPS]
relationship: part_of PSI:1000455 ! Ion Selection Description

[Term]
id: PSI:1000042
name: Intensity
def: "Intensity of ions as measured by the height or area of a peak in a mass spectrum." [PSI:GPS]
relationship: part_of PSI:1000455 ! Ion Selection Description

[Term]
id: PSI:1000043
name: Intensity Unit
def: "Intensity units are commonly arbitrary. Detected in counts per second (cps) when using counting detectors, but measured in volts when using analog detectors." [PSI:GPS]
is_a: PSI:1000460 ! Unit
relationship: part_of PSI:1000455 ! Ion Selection Description

[Term]
id: PSI:1000044
name: Activation Method
def: "Fragmentation method used for dissociation or fragmentation." [PSI:GPS]
relationship: part_of PSI:1000456 ! Precursor Activation Description

[Term]
id: PSI:1000045
name: Collision Energy
def: "Energy for an ion experiencing collision with a stationary gas particle resulting in dissociation of the ion. Projectile ions" [PSI:GPS]
relationship: part_of PSI:1000456 ! Precursor Activation Description

[Term]
id: PSI:1000046
name: Energy Unit
def: "Energy units are represented in either eV or Joules." [PSI:GPS]
is_a: PSI:1000460 ! Unit
relationship: part_of PSI:1000456 ! Precursor Activation Description

[Term]
id: PSI:1000047
name: Emulsion
def: "State if the sample is in emulsion form." [PSI:GPS]
is_a: PSI:1000003 ! Sample State

[Term]
id: PSI:1000048
name: Gas
def: "State if the sample is in gaseous form." [PSI:GPS]
is_a: PSI:1000003 ! Sample State

[Term]
id: PSI:1000049
name: Liquid
def: "State if the sample is in liquid form." [PSI:GPS]
is_a: PSI:1000003 ! Sample State

[Term]
id: PSI:1000050
name: Solid
def: "State if the sample is in solid form." [PSI:GPS]
is_a: PSI:1000003 ! Sample State

[Term]
id: PSI:1000051
name: Solution
def: "State if the sample is in solution form." [PSI:GPS]
is_a: PSI:1000003 ! Sample State

[Term]
id: PSI:1000052
name: Suspension
def: "State if the sample is in suspension form." [PSI:GPS]
is_a: PSI:1000003 ! Sample State

[Term]
id: PSI:1000053
name: Batch
def: "Sample batch lot identifier." [PSI:GPS]
is_a: PSI:1000007 ! Inlet Type

[Term]
id: PSI:1000054
name: Chromatography
def: "Chromatographic conditions used to obtain the sample." [PSI:GPS]
is_a: PSI:1000007 ! Inlet Type

[Term]
id: PSI:1000055
name: Continuous Flow Fast Atom Bombardment
def: "Fast atom bombardment ionization in which the analyte in solution is entrained in a flowing liquid matrix." [PSI:GPS]
exact_synonym: "CF-FAB" []
is_a: PSI:1000007 ! Inlet Type

[Term]
id: PSI:1000056
name: Direct
def: "The sample is directly inserted into the ion source, usually on the end of a heatable probe." [PSI:GPS]
is_a: PSI:1000007 ! Inlet Type

[Term]
id: PSI:1000057
name: Electrospray Inlet
def: "Inlet used for introducing the liquid sample into an electrospray ionization source." [PSI:GPS]
is_a: PSI:1000007 ! Inlet Type

[Term]
id: PSI:1000058
name: Flow Injection Analysis
def: "Sample is directly injected or infused into the ionization source." [PSI:GPS]
is_a: PSI:1000007 ! Inlet Type

[Term]
id: PSI:1000059
name: Inductively Coupled Plasma
def: "A gas discharge ion source in which the energy to the plasma is supplied by electromagnetic induction." [PSI:GPS]
is_a: PSI:1000007 ! Inlet Type

[Term]
id: PSI:1000060
name: Infusion
def: "The continuous flow of solution of a sample into the ionization source." [PSI:GPS]
is_a: PSI:1000007 ! Inlet Type

[Term]
id: PSI:1000061
name: Jet Separator
def: "A device that separates carrier gas from gaseous analyte molecules on the basis of diffusivity." [PSI:GPS]
is_a: PSI:1000007 ! Inlet Type

[Term]
id: PSI:1000062
name: Membrane Separator
def: "A device to separate carrier molecules from analyte molecules on the basis of ease of diffusion across a semipermeable membrane." [PSI:GPS]
is_a: PSI:1000007 ! Inlet Type

[Term]
id: PSI:1000063
name: Moving Belt
def: "Continuous moving surface in the form of a belt which passes through an ionsource carrying analyte molecules." [PSI:GPS]
is_a: PSI:1000007 ! Inlet Type

[Term]
id: PSI:1000064
name: Moving Wire
def: "Continuous moving surface in the form of a wire which passes through an ionsource carrying analyte molecules." [PSI:GPS]
is_a: PSI:1000007 ! Inlet Type

[Term]
id: PSI:1000065
name: Open Split
def: "A division of flowing stream of liquid into two streams." [PSI:GPS]
is_a: PSI:1000007 ! Inlet Type

[Term]
id: PSI:1000066
name: Particle Beam
def: "Method for generating ions from a solution of an analyte." [PSI:GPS]
is_a: PSI:1000007 ! Inlet Type

[Term]
id: PSI:1000067
name: Reservoir
def: "A sample inlet method involving a reservoir." [PSI:GPS]
is_a: PSI:1000007 ! Inlet Type

[Term]
id: PSI:1000068
name: Septum
def: "A disc composed of a flexible material that seals the entrance to the reservoir. Can also be enterance to the vaccum chamber." [PSI:GPS]
is_a: PSI:1000007 ! Inlet Type

[Term]
id: PSI:1000069
name: Thermospray Inlet
def: "A method for generating gas phase ions from a solution of an analyte by rapid heating of the sample." [PSI:GPS]
is_a: PSI:1000007 ! Inlet Type

[Term]
id: PSI:1000070
name: Atmospheric Pressure Chemical Ionization
def: "Chemical ionization that takes place at atmospheric pressure as opposed to the reduced pressure is normally used for chemical ionization." [PSI:GPS]
exact_synonym: "APCI" []
is_a: PSI:1000008 ! Ionization Type

[Term]
id: PSI:1000071
name: Chemical Ionization
def: "The formation of a new ion by the reaction of a neutral species with an ion. The process may involve transfer of an electron, a proton or other charged species between the reactants. When a positive ion results from chemical ionization the term may be used without qualification. When a negative ion results the term negative ion chemical ionization should be used. Note that this term is not synonymous with chemi-ionization.." [PSI:GPS]
exact_synonym: "CI" []
is_a: PSI:1000008 ! Ionization Type

[Term]
id: PSI:1000072
name: Electronic Ionization
def: "The ionization of an atom or molecule by electrons that are typically accelerated to energies between 50 and 150 eV. Usually 70 eV electrons are used to produce positive ions. The term 'electron impact' is not recommended." [PSI:GPS]
exact_synonym: "EI" []
is_a: PSI:1000008 ! Ionization Type

[Term]
id: PSI:1000073
name: Electrospray Ionization
def: "A process in which ionized species in the gas phase are produced from an analyte-containing solution via highly charged fine droplets, by means of spraying the solution from a narrow-bore needle tip at atmospheric pressure in the presence of a high electric field. When a pressurized gas is used to aid in the formation of a stable spray, the term pneumatically assisted electrospray ionization is used. The term ion spray is not recommended." [PSI:GPS]
exact_synonym: "ESI" []
is_a: PSI:1000008 ! Ionization Type

[Term]
id: PSI:1000074
name: Fast Atom Bombardment Ionization
def: "The ionization of any species by the interaction of a focused beam of neutral atoms having a translational energy of several thousand eV with a sample that is typically dissolved in a solvent matrix. See also secondary ionization." [PSI:GPS]
exact_synonym: "FAB" []
is_a: PSI:1000008 ! Ionization Type

[Term]
id: PSI:1000075
name: Matrix-assisted Laser Desorption Ionization
def: "The formation of gas-phase ions from molecules that are present in a solid or solvent matrix that is irradiated with a pulsed laser. See also laser desorption/ionization." [PSI:GPS]
exact_synonym: "MALDI" []
is_a: PSI:1000008 ! Ionization Type

[Term]
id: PSI:1000076
name: Negative Ion Mode
def: "TODO: Add defintion." [PSI:GPS]
is_obsolete: true

[Term]
id: PSI:1000077
name: Positive Ion Mode
def: "TODO: Add definition." [PSI:GPS]
is_obsolete: true

[Term]
id: PSI:1000078
name: Axial Ejection Linear Ion Trap
def: "A linear ion trap mass spectrometer where ions are ejected along the axis of the analyzer." [PSI:GPS]
is_a: PSI:1000010 ! Analyzer Type

[Term]
id: PSI:1000079
name: Fourier Transform Ion Cyclotron Resonance Mass Spectrometer
def: "A mass spectrometer based on the principle of ion cyclotron resonance in which an ion in a magnetic field moves in a circular orbit at a frequency characteristic of its m/z value. Ions are excited to a coherent orbit using a pulse of radio frequency energy and their image charge is detected on receiver plates as a time domain signal. Fourier transformation of the time domain signal results in a frequency domain signal which is converted to a mass spectrum based in the inverse relationship between frequency and m/z." [PSI:GPS]
exact_synonym: "FT_ICR" []
is_a: PSI:1000010 ! Analyzer Type

[Term]
id: PSI:1000080
name: Magnetic Sector
def: "A device that produces a magnetic field perpendicular to a charged particle beam that deflects the beam to an extent that is proportional to the particle momentum per unit charge. For a monoenergetic beam, the deflection is proportional to m/z." [PSI:GPS]
is_a: PSI:1000010 ! Analyzer Type

[Term]
id: PSI:1000081
name: Quadrupole
def: "A mass spectrometer that consists of four parallel rods whose centers form the corners of a square and whose opposing poles are connected. The voltage applied to the rods is a superposition of a static potential and a sinusoidal radio frequency potential. The motion of an ion in the x and y dimensions is described by the Matthieu equation whose solutions show that ions in a particular m/z range can be transmitted along the z axis." [PSI:GPS]
is_a: PSI:1000010 ! Analyzer Type

[Term]
id: PSI:1000082
name: Quadrupole Ion Trap
def: "Quadrupole Ion Trap mass analyzer captures the ions in a three dimensional ion trap and then selectively ejects them by varying the RF and DC potentials." [PSI:GPS]
exact_synonym: "QIT" []
is_a: PSI:1000010 ! Analyzer Type

[Term]
id: PSI:1000083
name: Radial Ejection Linear Ion Trap
def: "A linear ion trap mass spectrometer where ions are ejected along the radius of the analyzer." [PSI:GPS]
is_a: PSI:1000010 ! Analyzer Type

[Term]
id: PSI:1000084
name: Time-of-flight
def: "An instrument that separates ions by m/z in a field-free region after acceleration to a fixed kinetic energy." [PSI:GPS]
exact_synonym: "TOF" []
is_a: PSI:1000010 ! Analyzer Type

[Term]
id: PSI:1000085
name: Baseline
def: "An attribute of resolution when recording the detector response in absence of the analyte." [PSI:GPS]
is_a: PSI:1000012 ! Resolution Method

[Term]
id: PSI:1000086
name: Full Width at Half-Maximum
def: "A measure of resolution represented as width of the peak at half peak height." [PSI:GPS]
exact_synonym: "FWHM" []
is_a: PSI:1000012 ! Resolution Method

[Term]
id: PSI:1000087
name: Ten Percent Valley
def: "An attribute of resolution when the ratio between adjacent signals is 10% of the signal height." [PSI:GPS]
is_a: PSI:1000012 ! Resolution Method

[Term]
id: PSI:1000088
name: Constant
def: "When resolution is constant with respect to m/z." [PSI:GPS]
is_a: PSI:1000013 ! Resolution Type

[Term]
id: PSI:1000089
name: Proportional
def: "When resolution is proportional with respect to m/z." [PSI:GPS]
is_a: PSI:1000013 ! Resolution Type

[Term]
id: PSI:1000090
name: Mass Scan
def: "A variation of instrument where a selected mass is scanned." [PSI:GPS]
is_a: PSI:1000017 ! Scan Function

[Term]
id: PSI:1000091
name: Selected Ion Detection
def: "Please see Single Ion Monitoring." [PSI:GPS]
is_a: PSI:1000017 ! Scan Function

[Term]
id: PSI:1000092
name: Down
def: "Direction of mass scan." [PSI:GPS]
is_a: PSI:1000018 ! Scan Direction

[Term]
id: PSI:1000093
name: Up
def: "Direction of mass scan." [PSI:GPS]
is_a: PSI:1000018 ! Scan Direction

[Term]
id: PSI:1000094
name: Exponential
def: "The mass scan is done in exponential mode." [PSI:GPS]
is_a: PSI:1000019 ! Scan Law

[Term]
id: PSI:1000095
name: Linear
def: "The mass scan is done in linear mode." [PSI:GPS]
is_a: PSI:1000019 ! Scan Law

[Term]
id: PSI:1000096
name: Quadratic
def: "The mass scan is done in quadratic mode." [PSI:GPS]
is_a: PSI:1000019 ! Scan Law

[Term]
id: PSI:1000097
name: Constant Neutral Mass Loss
def: "A spectrum formed of all product ions that have been produced with a selected m/z decrement from any precursor ions. The spectrum shown correlates to the precursor ion spectrum. See also neutral loss spectrum." [PSI:GPS]
is_a: PSI:1000020 ! Tandem Scanning Method

[Term]
id: PSI:1000098
name: Multiple Ion Monitoring
def: "Data acquired when monitoring the ion current of a few specific m/z values." [PSI:GPS]
is_a: PSI:1000020 ! Tandem Scanning Method

[Term]
id: PSI:1000099
name: Multiple Reaction Monitoring
def: "This term is not recommended. See Selected Reaction Monitoring." [PSI:GPS]
exact_synonym: "MRM" []
is_a: PSI:1000020 ! Tandem Scanning Method

[Term]
id: PSI:1000100
name: Precursor Ion Scan
def: "The specific scan function or process that will record a precursor ion spectrum." [PSI:GPS]
is_a: PSI:1000020 ! Tandem Scanning Method

[Term]
id: PSI:1000101
name: Product Ion Scan
def: "The specific scan function or process that records product ion spectrum." [PSI:GPS]
is_a: PSI:1000020 ! Tandem Scanning Method

[Term]
id: PSI:1000102
name: Single Ion Monitoring
def: "The operation of a mass spectrometer to monitor a single ion rather than scanning entire mass spectrum." [PSI:GPS]
is_a: PSI:1000020 ! Tandem Scanning Method

[Term]
id: PSI:1000103
name: Single Reaction Monitoring
def: "See Selected Reaction Monitoring." [PSI:GPS]
is_a: PSI:1000020 ! Tandem Scanning Method

[Term]
id: PSI:1000104
name: None
def: "None." [PSI:GPS]
is_a: PSI:1000021 ! Reflectron State

[Term]
id: PSI:1000105
name: Off
def: "Off." [PSI:GPS]
is_a: PSI:1000021 ! Reflectron State

[Term]
id: PSI:1000106
name: On
def: "On." [PSI:GPS]
is_a: PSI:1000021 ! Reflectron State

[Term]
id: PSI:1000107
name: Channeltron
def: "A horn-shaped continuous dynode particle multiplier. The ion strikes the inner surface of the device and induces the production of secondary electrons that in turn impinge on the inner surfaces to produce more secondary electrons. This avalanche effect produces an increase in signal in the final measured current pulse. (Note that the " [PSI:GPS]
exact_synonym: "Channeltron Detector" []
is_a: PSI:1000026 ! Detector Type

[Term]
id: PSI:1000108
name: Conversion Dynode Electron Multiplier
def: "A surface that is held at high potential so that ions striking the surface produce electrons that are subsequently detected.\n" [PSI:GPS]
is_a: PSI:1000026 ! Detector Type

[Term]
id: PSI:1000109
name: Conversion Dynode Photomultiplier
def: "A detector in which ions strike a conversion dynode to produce electrons that in turn generate photons through a phosphorescent screen that are detected by a photomultiplier." [PSI:GPS]
is_a: PSI:1000026 ! Detector Type

[Term]
id: PSI:1000110
name: Daly Detector
def: "A metal knob held at high potential that emits secondary electrons when ions impinge on the surface. The secondary electrons are accelerated onto a scintillator that produces light that is then detected by a photomultiplier detector." [PSI:GPS]
exact_synonym: "Daly" []
is_a: PSI:1000026 ! Detector Type

[Term]
id: PSI:1000111
name: Electron Multiplier Tube
def: "A series of biased dynodes ejects secondary electrons when struck by an ion." [PSI:GPS]
exact_synonym: "EMT" []
is_a: PSI:1000026 ! Detector Type

[Term]
id: PSI:1000112
name: Faraday Cup
def: "A conducting cup or chamber that intercepts a charged particle beam and is electrically connected to a current measuring device." [PSI:GPS]
is_a: PSI:1000026 ! Detector Type

[Term]
id: PSI:1000113
name: Focal Plane Array
def: "A detector for spatially disperse ion beams in which all ions simultaneously impinge on the detector plane." [PSI:GPS]
is_a: PSI:1000026 ! Detector Type

[Term]
id: PSI:1000114
name: Microchannel Plate Detector
def: "A thin plate that contains a closely spaced array of channels that each act as a continuous dynode particle multiplier. A charged particle, fast neutral particle, or photon striking the plate causes a cascade of secondary electrons that ultimately exits the opposite side of the plate." [PSI:GPS]
exact_synonym: "Microchannel Plate Detector" []
is_a: PSI:1000026 ! Detector Type

[Term]
id: PSI:1000115
name: Multi-Collector
def: "A detector system commonly used in inductively coupled plasma mass spectrometers." [PSI:GPS]
is_a: PSI:1000026 ! Detector Type

[Term]
id: PSI:1000116
name: Photomultiplier
def: "A detector for conversion of the ion/electron signal into photon(s) which are then amplified and detected." [PSI:GPS]
exact_synonym: "PMT" []
is_a: PSI:1000026 ! Detector Type

[Term]
id: PSI:1000117
name: Analog-Digital Converter
def: "A detector acquisition mode that uses an ADC to converts voltage to a binary digital number." [PSI:GPS]
exact_synonym: "ADC" []
is_a: PSI:1000027 ! Detector Acquisition Mode

[Term]
id: PSI:1000118
name: Pulse Counting
def: "Pulse counting." [PSI:GPS]
is_a: PSI:1000027 ! Detector Acquisition Mode

[Term]
id: PSI:1000119
name: Time-Digital Converter
def: "A device for converting a signal of sporadic pluses into a digital representation of their time indices." [PSI:GPS]
exact_synonym: "TDC" []
is_a: PSI:1000027 ! Detector Acquisition Mode

[Term]
id: PSI:1000120
name: Transient Recorder
def: "A detector acquisition mode used for detecting transient signals." [PSI:GPS]
is_a: PSI:1000027 ! Detector Acquisition Mode

[Term]
id: PSI:1000121
name: ABI / SCIEX
def: "Applied Biosystems/MDS SCIEX Joint Venture" [PSI:GPS]
is_a: PSI:1000030 ! Vendor

[Term]
id: PSI:1000122
name: Bruker Daltonics
def: "Bruker Daltonics" [PSI:GPS]
is_a: PSI:1000030 ! Vendor

[Term]
id: PSI:1000123
name: Ion Spec
def: "IonSpec corporation" [PSI:GPS]
is_a: PSI:1000030 ! Vendor

[Term]
id: PSI:1000124
name: Shimadzu
def: "Shimadzu corporation" [PSI:GPS]
is_a: PSI:1000030 ! Vendor

[Term]
id: PSI:1000125
name: ThermoFinnigan
def: "ThermoFinnigan from Thermo Electron Corporation" [PSI:GPS]
is_a: PSI:1000030 ! Vendor

[Term]
id: PSI:1000126
name: Waters
def: "Waters Corporation" [PSI:GPS]
is_a: PSI:1000030 ! Vendor

[Term]
id: PSI:1000127
name: Centroid Mass Spectrum
def: "TODO: Add definition." [PSI:GPS]
is_a: PSI:1000035 ! Peak Processing

[Term]
id: PSI:1000128
name: Continuum Mass Spectrum
def: "TODO: Add definition." [PSI:GPS]
is_a: PSI:1000035 ! Peak Processing

[Term]
id: PSI:1000129
name: Negative
def: "Negative." [PSI:GPS]
is_a: PSI:1000037 ! Polarity
is_a: PSI:1000465 ! Polarity Mode

[Term]
id: PSI:1000130
name: Positive
def: "Positive." [PSI:GPS]
is_a: PSI:1000037 ! Polarity
is_a: PSI:1000465 ! Polarity Mode

[Term]
id: PSI:1000131
name: Number Of Counts
def: "TODO: Add definition." [PSI:GPS]
is_a: PSI:1000043 ! Intensity Unit

[Term]
id: PSI:1000132
name: Percent Of Base Peak
def: "TODO: Add definition." [PSI:GPS]
is_a: PSI:1000043 ! Intensity Unit

[Term]
id: PSI:1000133
name: Collision-Induced Dissociation
def: "The dissociation of an ion after collisional excitation. The term collisional-activated dissociation is not recommended." [PSI:GPS]
exact_synonym: "CID" []
is_a: PSI:1000044 ! Activation Method

[Term]
id: PSI:1000134
name: Plasma Desorption
def: "The ionization of material in a solid sample by bombarding it with ionic or neutral atoms formed as a result of the fission of a suitable nuclide, typically 252Cf. Synonymous with fission fragment ionization." [PSI:GPS]
exact_synonym: "PD" []
is_a: PSI:1000044 ! Activation Method

[Term]
id: PSI:1000135
name: Post-Source Decay
def: "A technique specific to reflectron time-of-flight mass spectrometers where product ions of metastable transitions or collision-induced dissociations generated in the drift tube prior to entering the reflectron are m/z separated to yield product ion spectra." [PSI:GPS]
exact_synonym: "PSD" []
is_a: PSI:1000044 ! Activation Method

[Term]
id: PSI:1000136
name: Surface-Induced Dissociation
def: "Fragmentation that results from the collision of an ion with a surface." [PSI:GPS]
exact_synonym: "SID" []
is_a: PSI:1000044 ! Activation Method

[Term]
id: PSI:1000137
name: Electron Volt
def: "A non-SI unit of energy (eV) defined as the energy acquired by a particle containing one unit of charge through a potential difference of one volt. An electron-volt is equal to 1.602 176 53(14) x 10^-19 J." [PSI:GPS]
exact_synonym: "eV" []
is_a: PSI:1000046 ! Energy Unit

[Term]
id: PSI:1000138
name: Percent
def: "TODO: Add definition." [PSI:GPS]
is_a: PSI:1000046 ! Energy Unit

[Term]
id: PSI:1000139
name: 4000 Q TRAP
def: "Applied Biosystems/MDS SCIEX Q 4000 TRAP MS" [PSI:GPS]
is_a: PSI:1000031 ! Model

[Term]
id: PSI:1000140
name: 4700 Proteomic Analyzer
def: "Applied Biosystems/MDS SCIEX 4700 Proteomic Analyzer MS" [PSI:GPS]
is_a: PSI:1000031 ! Model

[Term]
id: PSI:1000141
name: APEX IV
def: "Bruker Daltonics APEX IV MS" [PSI:GPS]
is_a: PSI:1000031 ! Model

[Term]
id: PSI:1000142
name: APEX-Q
def: "Bruker Daltonics APEX-Q MS" [PSI:GPS]
is_a: PSI:1000031 ! Model

[Term]
id: PSI:1000143
name: API 150EX
def: "Applied Biosystems/MDS SCIEX API 150EX MS" [PSI:GPS]
is_a: PSI:1000031 ! Model

[Term]
id: PSI:1000144
name: API 150EX Prep
def: "Applied Biosystems/MDS SCIEX API 150EX Prep MS" [PSI:GPS]
is_a: PSI:1000031 ! Model

[Term]
id: PSI:1000145
name: API 2000
def: "Applied Biosystems/MDS SCIEX API 2000 MS" [PSI:GPS]
is_a: PSI:1000031 ! Model

[Term]
id: PSI:1000146
name: API 3000
def: "Applied Biosystems/MDS SCIEX API 3000 MS" [PSI:GPS]
is_a: PSI:1000031 ! Model

[Term]
id: PSI:1000147
name: API 4000
def: "Applied Biosystems/MDS SCIEX API 4000 MS" [PSI:GPS]
is_a: PSI:1000031 ! Model

[Term]
id: PSI:1000148
name: autoFlex II
def: "Bruker Daltonics autoFlex II MS" [PSI:GPS]
is_a: PSI:1000031 ! Model

[Term]
id: PSI:1000149
name: autoFlex TOF/TOF
def: "Bruker Daltonics autoFlex TOF/TOF MS" [PSI:GPS]
is_a: PSI:1000031 ! Model

[Term]
id: PSI:1000150
name: Auto Spec Ultima NT
def: "Waters AutoSpec Ultima NT MS" [PSI:GPS]
is_a: PSI:1000031 ! Model

[Term]
id: PSI:1000151
name: Bio TOF II
def: "Bruker Daltonics BioTOF II MS" [PSI:GPS]
is_a: PSI:1000031 ! Model

[Term]
id: PSI:1000152
name: Bio TOF Q
def: "Bruker Daltonics BioTOF Q MS" [PSI:GPS]
is_a: PSI:1000031 ! Model

[Term]
id: PSI:1000153
name: DELTA plusAdvantage
def: "ThermoFinnigan DELTAplusAdvantage MS" [PSI:GPS]
is_a: PSI:1000031 ! Model

[Term]
id: PSI:1000154
name: DELTAplusXP
def: "ThermoFinnigan DELTAplusXP MS" [PSI:GPS]
is_a: PSI:1000031 ! Model

[Term]
id: PSI:1000155
name: ELEMENT2
def: "ThermoFinnigan ELEMENT2 MS" [PSI:GPS]
is_a: PSI:1000031 ! Model

[Term]
id: PSI:1000156
name: esquire4000
def: "Bruker Daltonics esquire4000 MS" [PSI:GPS]
is_a: PSI:1000031 ! Model

[Term]
id: PSI:1000157
name: esquire6000
def: "Bruker Daltonics esquire6000 MS" [PSI:GPS]
is_a: PSI:1000031 ! Model

[Term]
id: PSI:1000158
name: Explorer
def: "IonSpec Explorer MS" [PSI:GPS]
is_a: PSI:1000031 ! Model

[Term]
id: PSI:1000159
name: GCT
def: "Waters GCT MS" [PSI:GPS]
is_a: PSI:1000031 ! Model

[Term]
id: PSI:1000160
name: HCT
def: "Bruker Daltonics HCT MS" [PSI:GPS]
is_a: PSI:1000031 ! Model

[Term]
id: PSI:1000161
name: HCT Plus
def: "Bruker Daltonics HCTPlus MS" [PSI:GPS]
is_a: PSI:1000031 ! Model

[Term]
id: PSI:1000162
name: HiRes ESI
def: "IonSpec HiResESI MS" [PSI:GPS]
is_a: PSI:1000031 ! Model

[Term]
id: PSI:1000163
name: HiRes MALDI
def: "IonSpec HiResMALDI MS" [PSI:GPS]
is_a: PSI:1000031 ! Model

[Term]
id: PSI:1000164
name: IsoPrime
def: "Waters IsoPrime MS" [PSI:GPS]
is_a: PSI:1000031 ! Model

[Term]
id: PSI:1000165
name: IsoProbe
def: "Waters IsoProbe MS" [PSI:GPS]
is_a: PSI:1000031 ! Model

[Term]
id: PSI:1000166
name: IsoProbe T
def: "Waters IsoProbe T MS" [PSI:GPS]
is_a: PSI:1000031 ! Model

[Term]
id: PSI:1000167
name: LCQ Advantage
def: "ThermoFinnigan LCQ Advantage MS" [PSI:GPS]
is_a: PSI:1000031 ! Model

[Term]
id: PSI:1000168
name: LCQ Classic
def: "ThermoFinnigan LCQ Classic MS" [PSI:GPS]
is_a: PSI:1000031 ! Model

[Term]
id: PSI:1000169
name: LCQ Deca XP Plus
def: "ThermoFinnigan LCQ Deca XP Plus MS" [PSI:GPS]
is_a: PSI:1000031 ! Model

[Term]
id: PSI:1000170
name: M@LDI L
def: "Waters M@LDI L MS" [PSI:GPS]
is_a: PSI:1000031 ! Model

[Term]
id: PSI:1000171
name: M@LDI LR
def: "Waters M@LDI LR MS" [PSI:GPS]
is_a: PSI:1000031 ! Model

[Term]
id: PSI:1000172
name: MAT253
def: "ThermoFinnigan MAT253 MS" [PSI:GPS]
is_a: PSI:1000031 ! Model

[Term]
id: PSI:1000173
name: MAT900XP
def: "ThermoFinnigan MAT900XP MS" [PSI:GPS]
is_a: PSI:1000031 ! Model

[Term]
id: PSI:1000174
name: MAT900XP Trap
def: "ThermoFinnigan MAT900XP Trap MS" [PSI:GPS]
is_a: PSI:1000031 ! Model

[Term]
id: PSI:1000175
name: MAT95XP
def: "ThermoFinnigan MAT95XP MS" [PSI:GPS]
is_a: PSI:1000031 ! Model

[Term]
id: PSI:1000176
name: MAT95XP Trap
def: "ThermoFinnigan MAT95XP Trap MS" [PSI:GPS]
is_a: PSI:1000031 ! Model

[Term]
id: PSI:1000177
name: microFlex
def: "Bruker Daltonics microFlex MS" [PSI:GPS]
is_a: PSI:1000031 ! Model

[Term]
id: PSI:1000178
name: microTOFLC
def: "Bruker Daltonics microTOFLC MS" [PSI:GPS]
is_a: PSI:1000031 ! Model

[Term]
id: PSI:1000179
name: Neptune
def: "ThermoFinnigan NEPTUNE MS" [PSI:GPS]
is_a: PSI:1000031 ! Model

[Term]
id: PSI:1000180
name: NG-5400
def: "Waters NG-5400 MS" [PSI:GPS]
is_a: PSI:1000031 ! Model

[Term]
id: PSI:1000181
name: OMEGA
def: "IonSpec OMEGA MS" [PSI:GPS]
is_a: PSI:1000031 ! Model

[Term]
id: PSI:1000182
name: OMEGA-2001
def: "IonSpec OMEGA-2001 MS" [PSI:GPS]
is_a: PSI:1000031 ! Model

[Term]
id: PSI:1000183
name: OmniFlex
def: "Bruker Daltonics OminFlex MS" [PSI:GPS]
is_a: PSI:1000031 ! Model

[Term]
id: PSI:1000184
name: Platform ICP
def: "Waters Platform ICP MS" [PSI:GPS]
is_a: PSI:1000031 ! Model

[Term]
id: PSI:1000185
name: PolarisQ
def: "ThermoFinnigan PolarisQ MS" [PSI:GPS]
is_a: PSI:1000031 ! Model

[Term]
id: PSI:1000186
name: Proteomics Solution 1
def: "Applied Biosystems/MDS SCIEX Proteomics Solution 1 MS" [PSI:GPS]
is_a: PSI:1000031 ! Model

[Term]
id: PSI:1000187
name: Q TRAP
def: "Applied Biosystems/MDS SCIEX Q TRAP MS" [PSI:GPS]
is_a: PSI:1000031 ! Model

[Term]
id: PSI:1000188
name: Q-Tof micro
def: "Waters Q-Tof micro MS" [PSI:GPS]
is_a: PSI:1000031 ! Model

[Term]
id: PSI:1000189
name: Q-Tof Ultima
def: "Waters Q-Tof Ultima MS" [PSI:GPS]
is_a: PSI:1000031 ! Model

[Term]
id: PSI:1000190
name: QSTAR
def: "Applied Biosystems/MDS SCIEX QSTAR MS" [PSI:GPS]
is_a: PSI:1000031 ! Model

[Term]
id: PSI:1000191
name: Quattro micro
def: "Waters Quattro micro MS" [PSI:GPS]
is_a: PSI:1000031 ! Model

[Term]
id: PSI:1000192
name: Quattro UItima
def: "Waters Quattro Uitima MS" [PSI:GPS]
is_a: PSI:1000031 ! Model

[Term]
id: PSI:1000193
name: Surveyor MSQ
def: "ThermoFinnigan Surveyor MSQ MS" [PSI:GPS]
is_a: PSI:1000031 ! Model

[Term]
id: PSI:1000194
name: SymBiot I
def: "Applied Biosystems/MDS SCIEX SymBiot I MS" [PSI:GPS]
is_a: PSI:1000031 ! Model

[Term]
id: PSI:1000195
name: SymBiot XVI
def: "Applied Biosystems/MDS SCIEX SymBiot XVI MS" [PSI:GPS]
is_a: PSI:1000031 ! Model

[Term]
id: PSI:1000196
name: TEMPUS TOF
def: "ThermoFinnigan TEMPUS TOF MS" [PSI:GPS]
is_a: PSI:1000031 ! Model

[Term]
id: PSI:1000197
name: TRACE DSQ
def: "ThermoFinnigan TRACE DSQ MS" [PSI:GPS]
is_a: PSI:1000031 ! Model

[Term]
id: PSI:1000198
name: TRITON
def: "ThermoFinnigan TRITON MS" [PSI:GPS]
is_a: PSI:1000031 ! Model

[Term]
id: PSI:1000199
name: TSQ QUANTUM
def: "ThermoFinnigan TSQ QUANTUM MS" [PSI:GPS]
is_a: PSI:1000031 ! Model

[Term]
id: PSI:1000200
name: Ultima
def: "IonSpec Ultima MS" [PSI:GPS]
is_a: PSI:1000031 ! Model

[Term]
id: PSI:1000201
name: ultraFlex
def: "Bruker Daltonics ultraFlex MS" [PSI:GPS]
is_a: PSI:1000031 ! Model

[Term]
id: PSI:1000202
name: ultraFlex TOF/TOF
def: "Bruker Daltonics ultraFlex TOF/TOF MS" [PSI:GPS]
is_a: PSI:1000031 ! Model

[Term]
id: PSI:1000203
name: Voyager-DE PRO
def: "Applied Biosystems/MDS SCIEX Voyager-DE PRO MS" [PSI:GPS]
is_a: PSI:1000031 ! Model

[Term]
id: PSI:1000204
name: Voyager-DE STR
def: "Applied Biosystems/MDS SCIEX Voyager-DE STR MS" [PSI:GPS]
is_a: PSI:1000031 ! Model

[Term]
id: PSI:1000205
name: Selected Ion Monitoring
def: "The operation of a mass spectrometer in which the intensities of several specific m/z values are recorded rather than the entire mass spectrum." [PSI:GPS]
exact_synonym: "SIM" []
is_a: PSI:1000020 ! Tandem Scanning Method

[Term]
id: PSI:1000206
name: Selected Reaction Monitoring
def: "Data acquired from specific product ions corresponding to m/z selected precursor ions recorded via multiple stages of mass spectrometry. Selected reaction monitoring can be preformed in time or in space." [PSI:GPS]
exact_synonym: "SRM" []
is_a: PSI:1000020 ! Tandem Scanning Method

[Term]
id: PSI:1000207
name: Accurate Mass
def: "An experimentally determined mass that is can be to determine a unique elemental formula. For ions less than 200 u, a measurement with 5 ppm accuracy is sufficient to determine the elemental composition." [PSI:GPS]
relationship: part_of PSI:1000365 ! Ion

[Term]
id: PSI:1000208
name: Average Mass
def: "The mass of an ion or molecule calculated using the average mass of each element weighted for its natural isotopic abundance." [PSI:GPS]
relationship: part_of PSI:1000365 ! Ion

[Term]
id: PSI:1000209
name: Appearance Energy
def: "The minimum energy that must be imparted to an atom or molecule to produce a specified ion. The term appearance potential is not recommended." [PSI:GPS]
exact_synonym: "AE" []
relationship: part_of PSI:1000365 ! Ion

[Term]
id: PSI:1000210
name: Base Peak
def: "The peak in a mass spectrum that has the greatest intensity. This term may be applied to the spectra of pure substances or mixtures." [PSI:GPS]
exact_synonym: "BP" []
relationship: part_of PSI:1000442 ! Spectrum

[Term]
id: PSI:1000211
name: Charge Number
def: "The total charge on an ion divided by the electron charge e." [PSI:GPS]
exact_synonym: "z" []
relationship: part_of PSI:1000365 ! Ion

[Term]
id: PSI:1000212
name: Dalton
def: "A non-SI unit of mass (symbol Da) that is equal to the unified atomic mass unit: 1.660 538 86(28) x 10^-27 kg." [PSI:GPS]
exact_synonym: "Da" []
is_a: PSI:1000464 ! Mass Unit

[Term]
id: PSI:1000213
name: Electron Affinity
def: "The electron affinity of M is the minimum energy required for the process M- ? M + e where M- and M are in their ground rotational, vibrational and electronic states and the electron has zero kinetic energy." [PSI:GPS]
exact_synonym: "EA" []
relationship: part_of PSI:1000365 ! Ion

[Term]
id: PSI:1000214
name: Electron Energy
def: "The potential difference through which electrons are accelerated before they are used to bring about electron ionization." [PSI:GPS]
relationship: part_of PSI:1000458 ! Source Description

[Term]
id: PSI:1000215
name: Exact Mass
def: "The calculated mass of an ion or molecule containing a single isotope of each atom." [PSI:GPS]
relationship: part_of PSI:1000365 ! Ion

[Term]
id: PSI:1000216
name: Field-Free Region
def: "A section of a mass spectrometer in which there are no electric or magnetic fields." [PSI:GPS]
exact_synonym: "FFR" []
is_a: PSI:1000462 ! Ion Optic

[Term]
id: PSI:1000217
name: Ionization Cross Section
def: "The probability that a given ionization process will occur when an atom or molecule interacts with a photon, electron, atom or molecule." [PSI:GPS]
is_a: PSI:1000437 ! Ion Reaction Description

[Term]
id: PSI:1000218
name: Ioniazation Efficiency
def: "The ratio of the number of ions formed to the number of electrons, molecules or photons used. See Ionization Efficiency." [PSI:GPS]
is_obsolete: true

[Term]
id: PSI:1000219
name: Ionization Energy
def: "The minimum energy required to remove an electron from an atom or molecule to produce a positive ion." [PSI:GPS]
exact_synonym: "IE" []
relationship: part_of PSI:1000365 ! Ion

[Term]
id: PSI:1000220
name: Isotope Dilution Mass Spectrometry
def: "A quantitative mass spectrometry technique in which an isotopically enriched compound is used as an internal standard." [PSI:GPS]
exact_synonym: "IDMS" []
is_a: PSI:1000268 ! Mass Spectrometry

[Term]
id: PSI:1000221
name: Magnetic Deflection
def: "The deflection of charged particles in a magnetic field due to a force equal to qv  B where q is the particle charge, v its velocity and B the magnetic field. Magnetic deflection of an ion beam is used for m/z separation in a magnetic sector mass spectrometer." [PSI:GPS]
is_a: PSI:1000462 ! Ion Optic

[Term]
id: PSI:1000222
name: Mass Defect
def: "The difference between the monoisotipic and nominal mass of a molecule or atom." [PSI:GPS]
relationship: part_of PSI:1000365 ! Ion

[Term]
id: PSI:1000223
name: Mass Number
def: "The sum of the protons and neutrons in an atom, molecule or ion." [PSI:GPS]
relationship: part_of PSI:1000365 ! Ion

[Term]
id: PSI:1000224
name: Molecular Mass
def: "The mass of one mole of a molecular substance (6.022 1415(10) x 10^23 molecules)." [PSI:GPS]
relationship: part_of PSI:1000365 ! Ion

[Term]
id: PSI:1000225
name: Monoisotopic Mass
def: "The mass of an ion or molecule calculated using the mass of the most abundant isotope of each element." [PSI:GPS]
relationship: part_of PSI:1000365 ! Ion

[Term]
id: PSI:1000226
name: Molecular Beam Mass Spectrometry
def: "A mass spectrometry technique in which the sample is introduced into the mass spectrometer as a molecular beam." [PSI:GPS]
exact_synonym: "MBMS" []
is_a: PSI:1000293 ! Mass Spectrometer

[Term]
id: PSI:1000227
name: Multiphoton Ionization
def: "Photoionization of an atom or molecule in which in two or more photons are absorbed." [PSI:GPS]
exact_synonym: "MPI" []
relationship: part_of PSI:1000008 ! Ionization Type

[Term]
id: PSI:1000228
name: Nitrogen Rule
def: "An organic molecule containing the elements C, H, O, S, P, or halogen has an odd nominal mass if it contains an odd number of nitrogen atoms." [PSI:GPS]
is_a: PSI:1000437 ! Ion Reaction Description

[Term]
id: PSI:1000229
name: Nominal Mass
def: "The mass of an ion or molecule calculated using the mass of the most abundant isotope of each element rounded to the nearest integer value." [PSI:GPS]
relationship: part_of PSI:1000365 ! Ion

[Term]
id: PSI:1000230
name: Odd-Electron Rule
def: "Upon dissociation, odd-electron ions may form either odd or even-electron ions, whereras even-electron ions tend to form even-electron ions." [PSI:GPS]
is_a: PSI:1000437 ! Ion Reaction Description

[Term]
id: PSI:1000231
name: Peak
def: "A localized region of relatively large ion signal in a mass spectrum. Although peaks are often associated with particular ions, the terms peak and ion should not be used interchangeably." [PSI:GPS]
relationship: part_of PSI:1000442 ! Spectrum

[Term]
id: PSI:1000232
name: Peak Intensity
def: "The height or area of a peak in a mass spectrum." [PSI:GPS]
relationship: part_of PSI:1000231 ! Peak

[Term]
id: PSI:1000233
name: Proton Affinity
def: "The proton affinity of a species M is defined as the negative of the enthalpy change for the reaction M + H+ ? MH+." [PSI:GPS]
exact_synonym: "PA" [PSI:GPS]
relationship: part_of PSI:1000365 ! Ion

[Term]
id: PSI:1000234
name: Mass Resolving Power
def: "In a mass spectrum, the observed mass divided by the difference between two masses that can be separated: m/?m. The method by which ?m was obtained and the mass at which the measurement was made should be reported." [PSI:GPS]
is_a: PSI:1000444 ! m/z Separation Method

[Term]
id: PSI:1000235
name: Total Ion Chromatogram
def: "The chromatogram obtained by plotting the total ion current as a function of retention time." [PSI:GPS]
exact_synonym: "TIC" []
relationship: part_of PSI:1000461 ! Additional Description

[Term]
id: PSI:1000236
name: Transmission
def: "The ratio of the number of ions leaving a region of a mass spectrometer to the number entering that region." [PSI:GPS]
relationship: part_of PSI:1000451 ! Analyzer Description

[Term]
id: PSI:1000237
name: Unified Atomic Mass Unit
def: "A non-SI unit of mass (u) defined as one twelfth of ^12 C in its ground state and equal to 1.660 538 86(28) x 10^-27 kg." [PSI:GPS]
exact_synonym: "u" []
is_a: PSI:1000464 ! Mass Unit

[Term]
id: PSI:1000238
name: Accelerator Mass Spectrometry
def: "A mass spectrometry technique in which atoms extracted from a sample are ionized, accelerated to MeV energies and separated according to their momentum, charge and energy." [PSI:GPS]
exact_synonym: "AMS" []
is_a: PSI:1000293 ! Mass Spectrometer

[Term]
id: PSI:1000239
name: Atmospheric Pressure Matrix-Assisted Laser Desorption Ionization
def: "Matrix-assisted laser desorption ionization in which the sample target is at atmospheric pressure and the ions formed by the pulsed laser are sampled through a small aperture into the mass spectrometer." [PSI:GPS]
exact_synonym: "AP MALDI" []
is_a: PSI:1000008 ! Ionization Type

[Term]
id: PSI:1000240
name: Atmospheric Pressure Ionization
def: "Any ionization process in which ions are formed in the gas phase at atmospheric pressure." [PSI:GPS]
exact_synonym: "API" []
is_a: PSI:1000008 ! Ionization Type

[Term]
id: PSI:1000241
name: Atmostpheric Pressure Photoionization
def: "Atmospheric pressure chemical ionization in which the reactant ions are generated by photo-ionization." [PSI:GPS]
exact_synonym: "APPI" []
is_a: PSI:1000008 ! Ionization Type

[Term]
id: PSI:1000242
name: Blackbody Infrared Radiative Dissociation
def: "A special case of infrared multiphoton dissociation wherein excitation of the reactant ion is caused by absorption of infrared photons radiating from heated blackbody surroundings, which are usually the walls of a vacuum chamber. See also infrared multiphoton dissociation." [PSI:GPS]
exact_synonym: "BIRD" []
is_a: PSI:1000437 ! Ion Reaction Description
relationship: part_of PSI:1000456 ! Precursor Activation Description

[Term]
id: PSI:1000243
name: Charge-Remote Fragmentation
def: "A fragmentation of an even-electron ion in which the cleaved bond is not adjacent to the apparent charge site." [PSI:GPS]
exact_synonym: "CRF" []
is_a: PSI:1000437 ! Ion Reaction Description

[Term]
id: PSI:1000244
name: Consecutive Reaction Monitoring
def: "A type of MS/MS experiments with three or more stages of m/z separation and in which a particular multi-step reaction path is monitored." [PSI:GPS]
exact_synonym: "CRM" []
relationship: part_of PSI:1000456 ! Precursor Activation Description

[Term]
id: PSI:1000245
name: Charge Stripping
def: "The reaction of a positive ion with an atom or molecule that results in the removal of one or more electrons from the ion." [PSI:GPS]
exact_synonym: "CS" []
relationship: part_of PSI:1000456 ! Precursor Activation Description

[Term]
id: PSI:1000246
name: Delayed Extraction
def: "The application of the accelerating voltage pulse after a time delay in desorption ionization from a surface. The extraction delay can produce energy focusing in a time-of-flight mass spectrometer." [PSI:GPS]
exact_synonym: "DE" []
is_a: PSI:1000462 ! Ion Optic
relationship: part_of PSI:1000456 ! Precursor Activation Description

[Term]
id: PSI:1000247
name: Desorption Ionization
def: "The formation of ions from a solid or liquid material after the rapid vaporization of that sample." [PSI:GPS]
exact_synonym: "DI" []
is_a: PSI:1000008 ! Ionization Type

[Term]
id: PSI:1000248
name: Direct Insertion Probe
def: "A device for introducing a solid or liquid sample into a mass spectrometer ion source for desorption ionization." [PSI:GPS]
exact_synonym: "DIP" []
is_a: PSI:1000007 ! Inlet Type

[Term]
id: PSI:1000249
name: Direct Liquid Introduction
def: "The delivery of a liquid sample into a mass spectrometer for spray or desorption ionization." [PSI:GPS]
exact_synonym: "DLI" []
is_a: PSI:1000007 ! Inlet Type

[Term]
id: PSI:1000250
name: Electron Capture Dissociation
def: "A process in which a multiply protonated molecules interacts with a low energy electrons. Capture of the electron leads the liberation of energy and a reduction in charge state of the ion with the production of the (M + nH) (n-1)+ odd electron ion, which readily fragments." [PSI:GPS]
exact_synonym: "ECD" []
is_a: PSI:1000437 ! Ion Reaction Description
relationship: part_of PSI:1000456 ! Precursor Activation Description

[Term]
id: PSI:1000251
name: Even-Electron Ion
def: "An ion containing no unpaired electrons in its ground electronic state, e.g. CHv3^+." [PSI:GPS]
exact_synonym: "EE" []
is_a: PSI:1000365 ! Ion

[Term]
id: PSI:1000252
name: Electron-Induced Excitation in Organics
def: "The reaction of an ion with an electron in which the translational energy of the collision is converted into internal energy of the ion." [PSI:GPS]
exact_synonym: "EIEIO" []
is_a: PSI:1000437 ! Ion Reaction Description

[Term]
id: PSI:1000253
name: Electron Multiplier
def: "A device to amplify the current of a beam or packet of charged particles or photons by incidence upon the surface of an electrode to produce secondary electrons. The secondary electrons are then accelerated to other electrodes or parts of a continuous electrode to produce further secondary electrons." [PSI:GPS]
exact_synonym: "EM" []
is_a: PSI:1000026 ! Detector Type

[Term]
id: PSI:1000254
name: Electrostatic Energy Analyzer
def: "A device consisting of conducting parallel plates, concentric cylinders or concentric spheres that separates charged particles according to their kinetic energy by means of an electric field that is constant in time." [PSI:GPS]
exact_synonym: "ESA" []
is_a: PSI:1000443 ! Mass Analyzer

[Term]
id: PSI:1000255
name: Flowing Afterglow
def: "An ion source immersed in a flow of helium or other inert buffer gas that carries the ions through a meter-long reactor at pressures around 100 Pa." [PSI:GPS]
exact_synonym: "FA" []
is_a: PSI:1000008 ! Ionization Type

[Term]
id: PSI:1000256
name: High-field Asymmetric Waveform Ion Mobility Spectrometry
def: "The separation of ions between two concentric cylindrical electrodes due to application of a high voltage asymmetric waveform whereby ions migrate towards one of the two electrodes depending on the ratio of the high- to low-field mobility of the ion." [PSI:GPS]
exact_synonym: "FAIMS" []
is_a: PSI:1000293 ! Mass Spectrometer

[Term]
id: PSI:1000257
name: Field Desorption
def: "The formation of gas-phase ions from a material deposited on a solid surface in the presence of a high electric field. Because this process may encompass ionization by field ionization or other mechanisms, it is not recommended as a synonym for field desorption ionization." [PSI:GPS]
exact_synonym: "FD" []
is_a: PSI:1000008 ! Ionization Type

[Term]
id: PSI:1000258
name: Field Ionization
def: "The removal of electrons from any species by interaction with a high electric field." [PSI:GPS]
exact_synonym: "FI" []
is_a: PSI:1000008 ! Ionization Type

[Term]
id: PSI:1000259
name: Glow Discharge Ionization
def: "The formation of ions in the gas phase and from solid samples at the cathode by application of a voltage to a low pressure gas." [PSI:GPS]
exact_synonym: "GD-MS" []
is_a: PSI:1000008 ! Ionization Type

[Term]
id: PSI:1000260
name: Ion Kinetic Energy Spectrometry
def: "A method of analysis in which a beam of ions is separated according to the ratio of its translational energy to charge." [PSI:GPS]
exact_synonym: "IKES" []
is_a: PSI:1000293 ! Mass Spectrometer

[Term]
id: PSI:1000261
name: Ion Mobility Spectrometry
def: "The separation of ions according to their velocity through a buffer gas under the influence of an electric field." [PSI:GPS]
exact_synonym: "IMS" []
is_a: PSI:1000293 ! Mass Spectrometer

[Term]
id: PSI:1000262
name: Infrared Multiphoton Dissociation
def: "Multiphoton ionization ionization where the reactant ion dissociates as a result of the absorption of multiple infrared photons." [PSI:GPS]
exact_synonym: "IRMPD" []
relationship: part_of PSI:1000456 ! Precursor Activation Description

[Term]
id: PSI:1000263
name: Isotope Ratio Mass Spectrometry
def: "The measurement of the relative quantity of the different isotopes of an element in a material with a mass spectrometer." [PSI:GPS]
exact_synonym: "IRMS" []
is_a: PSI:1000268 ! Mass Spectrometry

[Term]
id: PSI:1000264
name: Ion Trap
def: "A device for spatially confining ions using electric and magnetic fields alone or in combination." [PSI:GPS]
exact_synonym: "IT" []
is_a: PSI:1000443 ! Mass Analyzer

[Term]
id: PSI:1000265
name: Kinetic Energy Release Distribution
def: "The distribution of kinetic energies of the products from dissociation of metastable ions." [PSI:GPS]
exact_synonym: "KERD" []
is_a: PSI:1000437 ! Ion Reaction Description

[Term]
id: PSI:1000266
name: Laser Desorption
def: "The formation of gas-phase neutral species by the interaction of a pulsed laser with a solid or liquid material." [PSI:GPS]
exact_synonym: "LD" []
is_a: PSI:1000008 ! Ionization Type

[Term]
id: PSI:1000267
name: Mass Analyzed Ion Kinetic Energy Spectrometry
def: "Spectra that are obtained from a sector mass spectrometer that incorporates at least one magnetic sector plus one electric sector in reverse geometry. The accelerating voltage, V, and the magnetic sector field, B, are set at fixed values to select the precursor ions, which are then allowed to dissociate or to react in a field free region between the two sectors. The kinetic energy product ions of m/z selected precursor ions is analyzed by scanning the electric sector field, E. The width of the product ion spectrum peaks is related to the kinetic energy release distribution (KERD) for the dissociation process." [PSI:GPS]
exact_synonym: "MIKES" []
is_a: PSI:1000293 ! Mass Spectrometer

[Term]
id: PSI:1000268
name: Mass Spectrometry
def: "The branch of science that deals with all aspects of mass spectrometers and the results obtained with these instruments." [PSI:GPS]
exact_synonym: "MS" []
relationship: part_of PSI:0000000 ! mzOntology

[Term]
id: PSI:1000269
name: Mass Spectrometry/Mass Spectrometry
def: "The acquisition, study and spectra of the electrically charged products or precursors of a m/z selected ion or ions." [PSI:GPS]
exact_synonym: "MS/MS" []
is_a: PSI:1000293 ! Mass Spectrometer

[Term]
id: PSI:1000270
name: Multiple Stage Mass Spectrometry
def: "Multiple stages of precursor ion m/z selection followed by product ion detection for successive progeny ions." [PSI:GPS]
exact_synonym: "MSn" []
is_a: PSI:1000445 ! Sequential m/z Separation Method

[Term]
id: PSI:1000271
name: Negative Ion Chemical Ionization
def: "Chemical ionization that results in the formation of negative ions." [PSI:GPS]
exact_synonym: "NICI" []
is_a: PSI:1000008 ! Ionization Type

[Term]
id: PSI:1000272
name: Neutralization Reionization Mass Spectrometry
def: "With this technique, m/z selected ions form neutrals by charge transfer to a collision gas or by dissociation. The neutrals are separated from the remaining ions and ionized in collisions with a second gas. This method is used to investigate reaction intermediates and other unstable species." [PSI:GPS]
exact_synonym: "NRMS" []
is_a: PSI:1000008 ! Ionization Type

[Term]
id: PSI:1000273
name: Photoionization
def: "The ionization of an atom or molecule by a photon, written M + h? ? M^+ + e. The term photon impact is not recommended." [PSI:GPS]
exact_synonym: "PI" []
is_a: PSI:1000008 ! Ionization Type

[Term]
id: PSI:1000274
name: Pyrolysis Mass Spectrometry
def: "A mass spectrometry technique in which the sample is heated to the point of decomposition and the gaseous decomposition products are introduced into the ion source." [PSI:GPS]
exact_synonym: "PyMS" []
is_a: PSI:1000008 ! Ionization Type

[Term]
id: PSI:1000275
name: Collision Quadrupole
def: "A transmission quadrupole to which an oscillating potential is applied so as to focus a beam of ions through a collision gas with no m/z separation." [PSI:GPS]
exact_synonym: "q" []
is_a: PSI:1000462 ! Ion Optic

[Term]
id: PSI:1000276
name: Resonance Enhanced Multiphoton Ionization
def: "Multiphoton ionization in which the ionization cross section is significantly enhanced because the energy of the incident photons is resonant with an intermediate excited state of the neutral species." [PSI:GPS]
exact_synonym: "REMPI" []
is_a: PSI:1000008 ! Ionization Type

[Term]
id: PSI:1000277
name: Residual Gas Analyzer
def: "A mass spectrometer used to measure the composition and pressure of gasses in an evacuated chamber." [PSI:GPS]
exact_synonym: "RGA" []
is_a: PSI:1000293 ! Mass Spectrometer

[Term]
id: PSI:1000278
name: Surface Enhanced Laser Desorption Ionization
def: "The formation of ionized species in the gas phase from analytes deposited on a particular surface substrate which is irradiated with a laser beam of which wavelength is absorbed by the surface. See also desorption/ionization on silicon and laser desorption/ionization." [PSI:GPS]
exact_synonym: "SELDI" []
is_a: PSI:1000008 ! Ionization Type

[Term]
id: PSI:1000279
name: Surface Enhanced Neat Desorption
def: "Matrix-assisted laser desorption ionization in which the matrix is covalently linked to the target surface." [PSI:GPS]
exact_synonym: "SEND" []
is_a: PSI:1000008 ! Ionization Type

[Term]
id: PSI:1000280
name: Suface Ionization
def: "The ionization of a neutral species when it interacts with a solid surface with an appropriate work function and temperature." [PSI:GPS]
exact_synonym: "SI" []
is_a: PSI:1000008 ! Ionization Type

[Term]
id: PSI:1000281
name: Selected Ion Flow Tube
def: "A device in which m/z selected ions are entrained in an inert carrier gas and undergo ion-molecule reactions." [PSI:GPS]
exact_synonym: "SIFT" []
is_a: PSI:1000462 ! Ion Optic

[Term]
id: PSI:1000282
name: Sustained Off-Resonance Irradiation
def: "A technique associated with Fourier transform ion cyclotron resonance (FT-ICR) mass spectrometry to carry out ion/neutral reactions such as low-energy collision-induced dissociation. A radio-frequency electric field of slightly off-resonance to the cyclotron frequency of the reactant ion cyclically accelerates and decelerates the reactant ion that is confined in the Penning ion trap. The ion's orbit does not exceed the dimensions of ion trap while the ion undergoes an ion/neutral species process that produces a high average translational energy for an extended time." [PSI:GPS]
exact_synonym: "SORI" []
is_a: PSI:1000044 ! Activation Method

[Term]
id: PSI:1000283
name: Spark Source Mass Spectrometry
def: "Mass spectrometry using spark ionization." [PSI:GPS]
exact_synonym: "SSMS" []
is_a: PSI:1000008 ! Ionization Type

[Term]
id: PSI:1000284
name: Stored Waveform Inverse Fourier Transform
def: "A technique to create excitation waveforms for ions in FT-ICR mass spectrometer or Paul ion trap. An excitation waveform in the time-domain is generated by taking the inverse Fourier transform of an appropriate frequency-domain programmed excitation spectrum, in which the resonance frequencies of ions to be excited are included. This technique may be used for selection of precursor ions in MS/MS experiments." [PSI:GPS]
exact_synonym: "SWIFT" []
is_a: PSI:1000443 ! Mass Analyzer

[Term]
id: PSI:1000285
name: Total Ion Current
def: "The sum of all the separate ion currents carried by the different ions contributing to a mass spectrum." [PSI:GPS]
exact_synonym: "TIC" []
is_a: PSI:1000026 ! Detector Type

[Term]
id: PSI:1000286
name: Time Lag Focusing
def: "Energy focusing in a time-of-flight mass spectrometer that is accomplished by introducing a time delay between the formation of the ions and the application of the accelerating voltage pulse." [PSI:GPS]
exact_synonym: "TLF" []
is_a: PSI:1000462 ! Ion Optic

[Term]
id: PSI:1000287
name: Time-Of-Flight Mass Spectrometer
def: "An instrument that separates ions by m/z in a field-free region after acceleration to a fixed kinetic energy." [PSI:GPS]
exact_synonym: "TOF-MS" []
is_a: PSI:1000293 ! Mass Spectrometer

[Term]
id: PSI:1000288
name: Cyclotron
def: "A device that uses an oscillating electric field parallel to a magnetic field to accelerate charged particles." [PSI:GPS]
is_a: PSI:1000443 ! Mass Analyzer

[Term]
id: PSI:1000289
name: Double-focusing Mass Spectrometer
def: "A mass spectrometer that uses a magnetic sector for m/z focusing and an electric sector for energy focusing of an ion beam." [PSI:GPS]
is_a: PSI:1000293 ! Mass Spectrometer

[Term]
id: PSI:1000290
name: Hybrid Mass Spectrometer
def: "A mass spectrometer that combines m/z analyzers of different types to perform tandem mass spectrometry." [PSI:GPS]
is_a: PSI:1000293 ! Mass Spectrometer

[Term]
id: PSI:1000291
name: Linear Ion Trap
def: "A two dimensional Paul ion trap in which ions are confined in the axial dimension by means of an electric field at the ends of the trap." [PSI:GPS]
is_a: PSI:1000443 ! Mass Analyzer

[Term]
id: PSI:1000292
name: Mass Spectrograph
def: "An instrument that separates a beam of ions according to their mass-to-charge ratio in which the ions are directed onto a focal plane detector such as a photographic plate." [PSI:GPS]
is_a: PSI:1000463 ! Instrument

[Term]
id: PSI:1000293
name: Mass Spectrometer
def: "An instrument that measures the mass-to-charge ratio and relative abundances of ions." [PSI:GPS]
is_a: PSI:1000463 ! Instrument

[Term]
id: PSI:1000294
name: Mass Spectrum
def: "A plot of the relative abundance of a beam or other collection of ions as a function of the mass-to-charge ratio (m/z)." [PSI:GPS]
is_a: PSI:1000442 ! Spectrum

[Term]
id: PSI:1000295
name: Mattauch-Herzog Geometry
def: "An arrangement for a double-focusing mass spectrometer in which a deflection of ?/(4 ?(2)) radians in a radial electric field is followed by a magnetic deflection of ?/2 radians." [PSI:GPS]
is_a: PSI:1000443 ! Mass Analyzer

[Term]
id: PSI:1000296
name: Nier-Johnson Geometry
def: "An arrangement for a double-focusing mass spectrometer in which a deflection of ?/2 radians in a radial electric field analyzer is followed by a magnetic deflection of ?/3 radians." [PSI:GPS]
is_a: PSI:1000443 ! Mass Analyzer

[Term]
id: PSI:1000297
name: Paul Ion Trap
def: "A device that permits the trapping of ions by means of an alternating current voltage. The ejection of ions with a m/z less than a prescribed value and retention of those with higher mass depends on the application of radio frequency voltages between a ring electrode and two end-cap electrodes to confine the ions in a circular path. The choice of these voltages determines the m/z below which ions are ejected." [PSI:GPS]
is_a: PSI:1000443 ! Mass Analyzer

[Term]
id: PSI:1000298
name: Prolate Traochoidal Mass Spectrometer
def: "A mass spectrometer in which the ions of different m/z are separated by means of crossed electric and magnetic fields in such a way that the selected ions follow a prolate trochoidal path." [PSI:GPS]
is_a: PSI:1000293 ! Mass Spectrometer

[Term]
id: PSI:1000299
name: Quistor
def: "An abbreviation of quadrupole ion storage trap. This term is synonymous with Paul Ion Trap." [PSI:GPS]
is_a: PSI:1000443 ! Mass Analyzer

[Term]
id: PSI:1000300
name: Reflectron
def: "A time-of-flight mass spectrometer that uses a static electric field to reverse the direction of travel of the ions entering it. A reflectron improves mass resolution by assuring that ions of the same m/z but different kinetic energy arrive at the detector at the same time." [PSI:GPS]
is_a: PSI:1000462 ! Ion Optic

[Term]
id: PSI:1000301
name: Sector Mass Spectrometer
def: "A mass spectrometer consisting of one or more magnetic sectors for m/z selection in a beam of ions. Such instruments may also have one or more electric sectors for energy selection." [PSI:GPS]
is_a: PSI:1000293 ! Mass Spectrometer

[Term]
id: PSI:1000302
name: Tandem Mass Spectrometer
def: "A mass spectrometer designed for mass spectrometry/mass spectrometry." [PSI:GPS]
is_a: PSI:1000293 ! Mass Spectrometer

[Term]
id: PSI:1000303
name: Transmission Quadrupole Mass Spectrometer
def: "A mass spectrometer that consists of four parallel rods whose centers form the corners of a square and whose opposing poles are connected. The voltage applied to the rods is a superposition of a static potential and a sinusoidal radio frequency potential. The motion of an ion in the x and y dimensions is described by the Matthieu equation whose solutions show that ions in a particular m/z range can be transmitted along the z axis." [PSI:GPS]
is_a: PSI:1000293 ! Mass Spectrometer

[Term]
id: PSI:1000304
name: Accelerating Voltage
def: "The electrical potential used to impart kinetic energy to ions in a mass spectrometer." [PSI:GPS]
is_a: PSI:1000462 ! Ion Optic

[Term]
id: PSI:1000305
name: Cyclotron Motion
def: "The circular motion of a charged particle moving at velocity v in a magnetic field B that results from the force qvB." [PSI:GPS]
is_a: PSI:1000444 ! m/z Separation Method

[Term]
id: PSI:1000306
name: Dynamic Mass Spectrometry
def: "A mass spectrometer in which m/z separation using one or more electric fields that vary with time." [PSI:GPS]
is_a: PSI:1000293 ! Mass Spectrometer

[Term]
id: PSI:1000307
name: Einzel Lens
def: "A three element charged particle lens in which the first and third elements are held at the same voltage. Such a lens produces focusing without changing the kinetic energy of the particle." [PSI:GPS]
is_a: PSI:1000462 ! Ion Optic

[Term]
id: PSI:1000308
name: Electric Field Strength
def: "The magnitude of the force per unit charge at a given point in space." [PSI:GPS]
is_a: PSI:1000462 ! Ion Optic

[Term]
id: PSI:1000309
name: First Stability Region
def: "The region of a Mathieu stability diagram closest to the origin. Ions within this region can traverse the full length of a transmission quadrupole." [PSI:GPS]
is_a: PSI:1000462 ! Ion Optic

[Term]
id: PSI:1000310
name: Fringing Field
def: "The electric or magnetic field that extends from the edge of a sector, lens or other ion optics element." [PSI:GPS]
is_a: PSI:1000462 ! Ion Optic

[Term]
id: PSI:1000311
name: Kinetic Energy Analyzer
def: "A device for measuring the kinetic energy of charged particles using a retarding field, time-of-flight, or the extent of deflection in an electric or magnetic field." [PSI:GPS]
is_a: PSI:1000462 ! Ion Optic

[Term]
id: PSI:1000312
name: Mass Limit
def: "The m/z value above which ions cannot be detected in a mass spectrometer." [PSI:GPS]
is_a: PSI:1000444 ! m/z Separation Method

[Term]
id: PSI:1000313
name: Mass Range
def: "The limit of m/z over which a mass spectrometer can detect ions." [PSI:GPS]
is_a: PSI:1000444 ! m/z Separation Method

[Term]
id: PSI:1000314
name: Mass Selective Axial Ejection
def: "The use of mass selective instability to eject ions of selected m/z values from an ion trap." [PSI:GPS]
is_a: PSI:1000444 ! m/z Separation Method

[Term]
id: PSI:1000315
name: Mass Selective Instability
def: "A method for selective ejection of ions according to their m/z value in an ion trap." [PSI:GPS]
is_a: PSI:1000444 ! m/z Separation Method

[Term]
id: PSI:1000316
name: Mathieu Stability Diagram
def: "A graphical representation expressed in terms of reduced coordinates that describes charged particle motion in a quadrupole mass filter or quadrupole ion trap mass spectrometer." [PSI:GPS]
is_a: PSI:1000444 ! m/z Separation Method

[Term]
id: PSI:1000317
name: Orthogonal Extraction
def: "The pulsed acceleration of ions perpendicular to their direction of travel into a time-of-flight mass spectrometer. Ions may be extracted from a directional ion source, drift tube or m/z separation stage." [PSI:GPS]
is_a: PSI:1000444 ! m/z Separation Method

[Term]
id: PSI:1000318
name: Resonance Ion Ejection
def: "A mode of ion ejection in a quadrupole ion trap that relies on a auxiliary radio frequency voltage that is applied to the end-cap electrodes. The voltage is tuned to the secular frequency of a particular ion to eject it." [PSI:GPS]
is_a: PSI:1000444 ! m/z Separation Method

[Term]
id: PSI:1000319
name: Space Charge Effect
def: "The mutual repulsion of particles of like charge that limits the current in a charged-particle beam and causes beams or packets of charged particles to expand radially over time." [PSI:GPS]
is_a: PSI:1000462 ! Ion Optic

[Term]
id: PSI:1000320
name: Static Field
def: "An electric or magnetic field that does not change in time." [PSI:GPS]
is_a: PSI:1000462 ! Ion Optic

[Term]
id: PSI:1000321
name: 2E Mass Spectrum
def: "A mass spectrum obtained by setting the electric sector field E to twice the value required to transmit the main ion-beam thereby allowing ions with a kinetic energy-to-charge ratio twice that of the main ion-beam to be transmitted. Product ions resulting from partial charge transfer reactions such as m^2+ + N ? m^+ + N^+ that occur in a collision cell (containing a gas, N) located in a field-free region preceding a magnetic and electric sector combination are detected. When the magnetic sector field B is scanned, a mass spectrum of singly charged product ions of doubly charged precursor ions is obtained." [PSI:GPS]
is_a: PSI:1000445 ! Sequential m/z Separation Method

[Term]
id: PSI:1000322
name: Charge Inversion Mass Spectrum
def: "The measurement of the relative abundance of ions that result from a charge inversion reaction as a function of m/z." [PSI:GPS]
is_a: PSI:1000294 ! Mass Spectrum

[Term]
id: PSI:1000323
name: Constant Neutral Loss Scan
def: "A scan designed to produce a constant neutral mass loss spectrum. Synonymous terms are constant neutral mass loss scan and fixed neutral fragment scan." [PSI:GPS]
is_a: PSI:1000441 ! Scan

[Term]
id: PSI:1000324
name: Constant Neutral Gain Scan
def: "A scan designed to produce a constant neutral gain spectrum." [PSI:GPS]
exact_synonym: "Constanst Neutral Mass Gain Scan" []
is_a: PSI:1000441 ! Scan

[Term]
id: PSI:1000325
name: Constant Neutral Mass Gain Spectrum
def: "A spectrum formed of all product ions that have been produced by gain of a pre-selected neutral mass following the reaction with and addition of the gas in a collision cell." [PSI:GPS]
is_a: PSI:1000294 ! Mass Spectrum

[Term]
id: PSI:1000326
name: Constant Neutral Mass Loss Spectrum
def: "A spectrum formed of all product ions that have been produced with a selected m/z decrement from any precursor ions. The spectrum shown correlates to the precursor ion spectrum. See also neutral loss spectrum." [PSI:GPS]
exact_synonym: "Constant Neutral Mass Loss" []
is_a: PSI:1000294 ! Mass Spectrum

[Term]
id: PSI:1000327
name: Consecutive Reaction Monitoring
def: "A type of MS/MS experiments with three or more stages of m/z separation and in which a particular multi-step reaction path is monitored." [PSI:GPS]
is_a: PSI:1000445 ! Sequential m/z Separation Method

[Term]
id: PSI:1000328
name: E/2 Mass Spectrum
def: "A mass spectrum obtained using a sector mass spectrometer in which the electric sector field E is set to half the value required to transmit the main ion-beam. This spectrum records the signal from doubly charged product ions of charge-stripping reactions." [PSI:GPS]
is_a: PSI:1000294 ! Mass Spectrum

[Term]
id: PSI:1000329
name: Linked Scan
def: "A scan in an instrument with two or more m/z analysers or in a sector mass spectrometer that incorporates at least one magnetic sector and one electric sector. Two or more of the analyzers are scanned simultaneously so as to preserve a predetermined relationship between scan parameters to produce a product ion, precursor ion or constant neutral loss spectrum." [PSI:GPS]
is_a: PSI:1000441 ! Scan

[Term]
id: PSI:1000330
name: Linked Scan at Constant B/E
def: "A linked scan at constant B/E may be performed on a sector mass spectrometer that incorporates at least one magnetic sector plus one electric sector. The magnetic field B and the electric field field E are scanned simultaneously while the accelerating voltage V is held constant, so as to maintain the ratio of the two fields constant. This linked scan may record a product ion spectrum of dissociation or other reactions occurring in a field free region preceding the two sectors." [PSI:GPS]
is_a: PSI:1000441 ! Scan

[Term]
id: PSI:1000331
name: Linked Scan at Constant E2/V
def: "A linked scan performed on a sector instrument that incorporates at least one electric sector plus one magnetic sector. The electric sector field, E, and the accelerating voltage, V, are scanned simultaneously, so as to maintain the ratio E2/V at a constant value. This linked scan recordss a product ion spectrum of dissociation or other reactions occurring in a field free region (FFR) preceding the two sectors. The term " [PSI:GPS]
is_a: PSI:1000441 ! Scan

[Term]
id: PSI:1000332
name: Linked Scan at Constant B2/E
def: "A linked scan performed on a sector mass spectrometer that incorporates at least one electric sector plus one magnetic sector in either order. The accelerating voltage is fixed and the magnetic field, B, and the electric field, E, are scanned simultaneously so as to maintain the ratio B2/E at a constant value. This linked scan records a precursor ion spectrum of dissociation or other reactions occurring in the field free region preceding the two sectors. The term B2/E linked scan is not recommended." [PSI:GPS]
is_a: PSI:1000441 ! Scan

[Term]
id: PSI:1000333
name: Linked Scan at Constant B[1-(E/E0)]^1/2 / E
def: "A linked scan performed on a sector instrument that incorporates at least one electric sector plus one magnetic sector placed in either order. The accelerating voltage is fixed while scanning the magnetic field, B, and electric field, E, simultaneously, so as to maintain the quantity B[1-(E/E0)]1/2/E at a constant value. This linked scan records a constant neutral mass loss (or gain) spectrum of dissociation or other reactions occurring in a field free region preceding the two sectors. E0 is the electric field required to transmit the singly charged analog of the desired neutral fragment. The term B[1-(E/E0)]1/2/E linked scan" [PSI:GPS]
is_a: PSI:1000441 ! Scan

[Term]
id: PSI:1000334
name: MS/MS in Time
def: "A tandem mass spectrometry method in which product ion spectra are recorded in a single m/z analyzer (such as a Paul Ion Trap or FTMS) in discreet steps over time. Ions in a specific m/z range are selected, dissociated, and the product ions analyzed sequentially in time." [PSI:GPS]
is_a: PSI:1000445 ! Sequential m/z Separation Method

[Term]
id: PSI:1000335
name: MS/MS in Space
def: "A tandem mass spectrometry method in which product ion spectra are recorded in m/z analyzers separated in space. Specific m/z separation functions are designed such that in one section of the instrument ions are selected, dissociated in an intermediate region, and the product ions are then transmitted to another analyser for m/z separation and data acquisition." [PSI:GPS]
is_a: PSI:1000445 ! Sequential m/z Separation Method

[Term]
id: PSI:1000336
name: Neutral Loss
def: "The the loss of an uncharged species during a rearrangement process." [PSI:GPS]
is_a: PSI:1000445 ! Sequential m/z Separation Method

[Term]
id: PSI:1000337
name: Nth Generation Product Ion
def: "The serial product ions from dissociation of selected precursor ions where n refers to the number of stages of dissociation. See also Progeny Ion." [PSI:GPS]
is_a: PSI:1000365 ! Ion

[Term]
id: PSI:1000338
name: Nth Generation Product Ion Scan
def: "The specific scan functions or processes that record the appropriate generation of product ion or ions of any m/z selected precursor ions." [PSI:GPS]
is_a: PSI:1000441 ! Scan

[Term]
id: PSI:1000339
name: Nth Generation Product Ion Spectrum
def: "The mass spectrum recorded from any  mass spectrometer in which the appropriate scan function can be set to record the appropriate generation product ion or ions of m/z selected precursor ions." [PSI:GPS]
is_a: PSI:1000343 ! Product Ion Spectrum

[Term]
id: PSI:1000340
name: Precursor Ion
def: "An ion that reacts to form particular product ions. The reaction can be unimolecular dissociation, ion/molecule reaction, isomerization, or change in charge state. The term parent ion is not recommended." [PSI:GPS]
is_a: PSI:1000365 ! Ion

[Term]
id: PSI:1000341
name: Precursor Ion Spectrum
def: "The mass spectrum recorded from any spectrometer in which the appropriate m/z separation function can be set to record the precursor ion or ions of selected product ions." [PSI:GPS]
is_a: PSI:1000294 ! Mass Spectrum

[Term]
id: PSI:1000342
name: Product Ion
def: "An ion formed as the product of a reaction involving a particular precursor ion. The reaction can unimolecular dissociation, an ion/molecule reaction, or involve simply a change in the number of charges. The terms daughter ion and parent ion are not recommended." [PSI:GPS]
is_a: PSI:1000365 ! Ion

[Term]
id: PSI:1000343
name: Product Ion Spectrum
def: "A mass spectrum recorded from any spectrometer in which the appropriate m/z separation scan function is set to record the product ion or ions of selected precursor ions." [PSI:GPS]
is_a: PSI:1000294 ! Mass Spectrum

[Term]
id: PSI:1000344
name: Progeny Ion
def: "A charged product of a series of consecutive reactions that includes product ions, 1st generation product ions, 2nd generation product ions, etc. Given the sequential fragmentation scheme: M1+ ? M2+ ? M3+ ? M4+ ? M5+ M4+ is the precursor ion of M5+, a 1st generation product ion of M3+, a 2nd generation product ion of M2+ and a 3rd generation product ion of M1+. " [PSI:GPS]
exact_synonym: "Progeny Fragment Ion" []
is_a: PSI:1000365 ! Ion

[Term]
id: PSI:1000345
name: Array Detector
def: "A detector composed of a number of ion collection elements or devices, arranged in a line or grid where each element is an individual detector." [PSI:GPS]
is_a: PSI:1000026 ! Detector Type

[Term]
id: PSI:1000346
name: Conversion Dynode
def: "A surface that is held at high potential such that ions striking the surface produce electrons that are subsequently detected." [PSI:GPS]
is_a: PSI:1000026 ! Detector Type

[Term]
id: PSI:1000347
name: Dynode
def: "One of a series of electrodes in a photomultiplier tube. Such an arrangement is able to amplify the current emitted by the photocathode." [PSI:GPS]
is_a: PSI:1000026 ! Detector Type

[Term]
id: PSI:1000348
name: Focal Plane Collector
def: "A detector for spatially disperse ion beams in which all ions simultaneously impinge on the detector plane." [PSI:GPS]
is_a: PSI:1000026 ! Detector Type

[Term]
id: PSI:1000349
name: Ion-to-Photon Detector
def: "A detector in which ions strike a conversion dynode to produce electrons that in turn strike a phosphor and the resulting photons are detected by a photomultiplier." [PSI:GPS]
is_a: PSI:1000026 ! Detector Type

[Term]
id: PSI:1000350
name: Point Collector
def: "A detector in which the ion beam is focused onto a point and the individual ions arrive sequentially." [PSI:GPS]
is_a: PSI:1000026 ! Detector Type

[Term]
id: PSI:1000351
name: Postacceleration Detector
def: "A detector in which the charged particles are accelerated to a high velocity and impinge on a conversion dynode, emitting secondary electrons. The electrons are accelerated onto a phosphor screen, which emits photons that are in turn detected using a photomultiplier or other photon detector." [PSI:GPS]
is_a: PSI:1000026 ! Detector Type

[Term]
id: PSI:1000352
name: Secondary Electron
def: "Electrons that are ejected from a sample surface as a result of bombardment by a primary beam of atoms, ions or photons." [PSI:GPS]
is_a: PSI:1000026 ! Detector Type

[Term]
id: PSI:1000353
name: Adduct Ion
def: "An ion formed by the interaction of an ion with one or more atoms or molecules to form an ion containing all the constituent atoms of the precursor ion as well as the additional atoms from the associated atoms or molecules." [PSI:GPS]
is_a: PSI:1000365 ! Ion

[Term]
id: PSI:1000354
name: Aromatic Ion
def: "A planar cyclic ion that obeys the the Hckel (4n + 2) rule where n is a positive integer representing the number of conjugated ? electrons. Charge delocalization leads to greater stability compared to a hypothetical localized structure." [PSI:GPS]
is_a: PSI:1000365 ! Ion

[Term]
id: PSI:1000355
name: Analog Ion
def: "Ions that have similar chemical valence, for example the acetyl cation CH3-CO+ and the thioacetyl cation CH3-CS+." [PSI:GPS]
is_a: PSI:1000365 ! Ion

[Term]
id: PSI:1000356
name: Anti-Aromatic Ion
def: "A planar cyclic ion with 4n ? electrons and is therefore not aromatic." [PSI:GPS]
is_a: PSI:1000365 ! Ion

[Term]
id: PSI:1000357
name: Cationized Molecule
def: "An ion formed by the association of a cation with a neutral molecule, M, for example [M+ Na]+ and [M + K]+. The terms quasi-molecular ion and pseudo-molecular ion should not be used. " [PSI:GPS]
is_a: PSI:1000365 ! Ion

[Term]
id: PSI:1000358
name: Cluster Ion
def: "An ion formed by a multi-component atomic or molecular assembly of one or more ions with atoms or molecules, such as [(H20)nH]+, [(NaCl)nNa]+ and [(H3PO3)nHPO3]-." [PSI:GPS]
is_a: PSI:1000365 ! Ion

[Term]
id: PSI:1000359
name: Conventional Ion
def: "A radical cation or anion in which the charge site and the unpaired electron spin are both formally located in the same atom or group of atoms, as opposed to the spatially separate electronic configuration of distonic ions. The radical cation of methanol, CH3OH+, in which the charge and spin sites are formally located at the O atom is an example of a conventional ion, whereas .CH2-OH2+ is a distonic ion." [PSI:GPS]
is_a: PSI:1000365 ! Ion

[Term]
id: PSI:1000360
name: Diagnostic Ion
def: "A product ion whose formation reveals structural or compositional information of its precursor. For instance, the phenyl cation in an electron ionization mass spectrum is a diagnostic ion for benzene and derivatives." [PSI:GPS]
is_a: PSI:1000365 ! Ion

[Term]
id: PSI:1000361
name: Dimeric Ion
def: "An ion formed by ionization of a dimer or by the association of an ion with its neutral counterpart such as [M2]+ or [M-H-M]+." [PSI:GPS]
is_a: PSI:1000365 ! Ion

[Term]
id: PSI:1000362
name: Distonic Ion
def: "A radical cation or anion in which the charge site and the unpaired electron spin cannot be both formally located in the same atom or group of atoms as it can be with a conventional ion. For example, CH2-OH2+ is a distonic ion whereas the radical cation of methanol, CH3OH+ is a conventional ion." [PSI:GPS]
is_a: PSI:1000365 ! Ion

[Term]
id: PSI:1000363
name: Enium Ion
def: "A positively charged lower-valency ion of the nonmetallic elements. The methenium ion is CH3+. Other examples are the oxenium, sulfenium, nitrenium, phosphenium, and halenium ions." [PSI:GPS]
is_a: PSI:1000365 ! Ion

[Term]
id: PSI:1000364
name: Fragment Ion
def: "A product ion resulting from the dissociation of a precursor ion." [PSI:GPS]
is_a: PSI:1000365 ! Ion

[Term]
id: PSI:1000365
name: Ion
def: "An atomic or molecular species having a net positive or negative electric charge." [PSI:GPS]
relationship: part_of PSI:0000000 ! mzOntology

[Term]
id: PSI:1000366
name: Isotopologue Ion
def: "An ion that differs only in the isotopic composition of one or more of its constituent atoms. For example CH4+. and CH3D+. or 10BF3 and 11BF3. The term isotopologue is a contraction of isotopic homologue." [PSI:GPS]
is_a: PSI:1000365 ! Ion

[Term]
id: PSI:1000367
name: Isotopomeric Ion
def: "An iIsomeric ion having the same number of each isotopic atom but differing in their positions. Isotopomeric ions can be either configurational isomers, e.g. the radical cations of dichloropyridines in which 35Cl and 37Cl exchange positions or isotopic stereoisomers, e.g. the radical cations of (R)- and (S)-CH3CHDOH or (Z)- and (E)-CH3CH=CHD. The term isotopomeric is a contraction of isotopic isomer." [PSI:GPS]
is_a: PSI:1000365 ! Ion

[Term]
id: PSI:1000368
name: Metastable Ion
def: "An ion that is formed with internal energy higher than the threshold for dissociation but with a lifetime great enough to allow it to exit the ion source and enter the mass spectrometer where it dissociates before detection." [PSI:GPS]
is_a: PSI:1000365 ! Ion

[Term]
id: PSI:1000369
name: Molecular Ion
def: "An ion formed by the removal of one or more electrons to form a positive ion or the addition off one or more electrons to form a negative ion." [PSI:GPS]
is_a: PSI:1000365 ! Ion

[Term]
id: PSI:1000370
name: Negative Ion
def: "An atomic or molecular species having a net negative electric charge." [PSI:GPS]
is_a: PSI:1000365 ! Ion

[Term]
id: PSI:1000371
name: Non-Classical Ion
def: "A penta-coordinated carbonium ion." [PSI:GPS]
is_a: PSI:1000365 ! Ion

[Term]
id: PSI:1000372
name: Onium Ion
def: "A positively charged hypervalent ion of the nonmetallic elements. Examples are the methonium ion CH5+, the hydrogenonium ion H3+ and and the hydronium ion H3O+. Other examples are the carbonium, oxonium, sulfonium, nitronium, diazonium, phosphonium, and halonium ions. Onium ions are not limited to monopositive ions; multiply-charged onium ions exist such as the gitonic (proximal) oxonium dication H4O2+ and the distonic oxonium dication H2O+-CH2-CH2-OH2+." [PSI:GPS]
is_a: PSI:1000365 ! Ion

[Term]
id: PSI:1000373
name: Principal Ion
def: "The most abundant ion of a group of isotopologue ions. For example, 11 B^79 Br2^81 Br+ is the principal ion of BBr3+." [PSI:GPS]
is_a: PSI:1000365 ! Ion

[Term]
id: PSI:1000374
name: Positive Ion
def: "An atomic or molecular species having a net positive electric charge." [PSI:GPS]
is_a: PSI:1000365 ! Ion

[Term]
id: PSI:1000375
name: Protonated Molecule
def: "An ion formed by interaction of a neutral molecule with a proton and represented by the symbol [M + H]+, where M is the neutral molecule. The term 'protonated molecular ion,' 'quasi-molecular ion' and 'pseudo-molecular ion' are not recommended." [PSI:GPS]
is_a: PSI:1000365 ! Ion

[Term]
id: PSI:1000376
name: Radical Ion
def: "An ion, either a cation or anion, containing unpaired electrons in its ground state. The unpaired electron is denoted by a superscript dot alongside the superscript symbol for charge, such as for the molecular ion of a molecule M, that is, M+. Radical ions with more than one charge and/or more than one unpaired electron are denoted such as M(2+)(2).Unless the positions of the unpaired electron and charge can be associated with specific atoms, superscript charge designation should be placed before the superscript dot designation." [PSI:GPS]
is_a: PSI:1000365 ! Ion

[Term]
id: PSI:1000377
name: Reference Ion
def: "A stable ion whose structure is known with certainty. These ions are usually formed by direct ionization of a neutral molecule of known structure and are used to verify by comparison the structure of an unknown ion." [PSI:GPS]
is_a: PSI:1000365 ! Ion

[Term]
id: PSI:1000378
name: Stable Ion
def: "An ion with internal energy sufficiently low that it does not rearrange or dissociate prior to detection in a mass spectrometer." [PSI:GPS]
is_a: PSI:1000365 ! Ion

[Term]
id: PSI:1000379
name: Unstable Ion
def: "An ion with sufficient enerrgy to dissociate within the ion source." [PSI:GPS]
is_a: PSI:1000365 ! Ion

[Term]
id: PSI:1000380
name: Adiabatic Ionization
def: "A process whereby an electron is removed from an atom, ion, or molecule to produce an ion in its lowest energy state." [PSI:GPS]
is_a: PSI:1000008 ! Ionization Type

[Term]
id: PSI:1000381
name: Associative Ionization
def: "An ionization process in which two excited atoms or molecules react to form a single positive ion and an electron." [PSI:GPS]
is_a: PSI:1000008 ! Ionization Type

[Term]
id: PSI:1000382
name: Atmospheric Pressure Photoionization
def: "Atmospheric pressure chemical ionization in which the reactant ions are generated by photo-ionization." [PSI:GPS]
is_a: PSI:1000008 ! Ionization Type

[Term]
id: PSI:1000383
name: Autodetachment
def: "The formation of a neutral when a negative ion in a disrtete state with an energy greater than the detachment threshold loses an electron spontaneously without further interaction with an energy source." [PSI:GPS]
is_a: PSI:1000008 ! Ionization Type

[Term]
id: PSI:1000384
name: Autoionization
def: "The formation of an ion when an atom or molecule in a discrete state with an energy greater than the ionization threshold loses an electron spontaneously without further interaction with an energy source." [PSI:GPS]
is_a: PSI:1000008 ! Ionization Type

[Term]
id: PSI:1000385
name: Charge Exchange Ionization
def: "The interaction of an ion with an atom or molecule in which the charge on the ion is transferred to the neutral without the dissociation of either. Synonymous with charge transfer ionization." [PSI:GPS]
is_a: PSI:1000008 ! Ionization Type

[Term]
id: PSI:1000386
name: Chemi-ionization
def: "The reaction of a neutral molecule with an internally excited molecule to form an ion. Note that this term is not synonymous with chemical ionization." [PSI:GPS]
is_a: PSI:1000008 ! Ionization Type

[Term]
id: PSI:1000387
name: Desorption/Ionization On Silicon
def: "The formation of ions by laser desorption ionization of a sample deposited on a porous silicon surface." [PSI:GPS]
is_a: PSI:1000008 ! Ionization Type

[Term]
id: PSI:1000388
name: Dissociative Ionization
def: "The reaction of a gas-phase molecule that results in its decomposition to form products, one of which is an ion." [PSI:GPS]
is_a: PSI:1000008 ! Ionization Type

[Term]
id: PSI:1000389
name: Electron Ionization
def: "The ionization of an atom or molecule by electrons that are typically accelerated to energies between 50 and 150 eV. Usually 70 eV electrons are used to produce positive ions. The term 'electron impact' is not recommended." [PSI:GPS]
is_a: PSI:1000008 ! Ionization Type

[Term]
id: PSI:1000390
name: Ion Desolvation
def: "The removal of solvent adducts from a gas phase adduct ion." [PSI:GPS]
is_a: PSI:1000437 ! Ion Reaction Description

[Term]
id: PSI:1000391
name: Ion-Pair Formation
def: "The reaction of a molecule to form both a positive ion and negative ion fragment among the products." [PSI:GPS]
is_a: PSI:1000437 ! Ion Reaction Description

[Term]
id: PSI:1000392
name: Ionization Efficiency
def: "The ratio of the number of ions formed to the number of electrons, molecules or photons used." [PSI:GPS]
relationship: part_of PSI:1000458 ! Source Description

[Term]
id: PSI:1000393
name: Laser Desorption Ionization
def: "The formation of gas-phase ions by the interaction of a pulsed laser with a solid or liquid material." [PSI:GPS]
is_a: PSI:1000008 ! Ionization Type

[Term]
id: PSI:1000394
name: Laser Ionization
def: "The formation of ions through the interaction of a laser with a material or with gas-phase ions or molecules." [PSI:GPS]
is_a: PSI:1000008 ! Ionization Type

[Term]
id: PSI:1000395
name: Liquid Secondary Ionization
def: "The ionization of any species by the interaction of a focused beam of ions with a sample that is dissolved in a solvent matrix. See also fast atom bombardment and secondary ionization." [PSI:GPS]
is_a: PSI:1000008 ! Ionization Type

[Term]
id: PSI:1000396
name: Membrane Inlet
def: "A semi-permeable membrane separator that permits the passage of gas sample directly to the mass spectrometer ion source." [PSI:GPS]
is_a: PSI:1000007 ! Inlet Type

[Term]
id: PSI:1000397
name: Microelectrospray
def: "Electrospray ionization at a solvent flow rate less than 1 ?L/min." [PSI:GPS]
is_a: PSI:1000008 ! Ionization Type

[Term]
id: PSI:1000398
name: Nanoelectrospray
def: "Electrospray ionization at a flow rate less than 100 nL/min. Nanoelectrospray is synonymous with nanospray. See also electrospray ionization and microelectrospray." [PSI:GPS]
is_a: PSI:1000008 ! Ionization Type

[Term]
id: PSI:1000399
name: Penning Ionization
def: "Ionization that occurs through the interaction of two or more neutral gaseous species, at least one of which is internally excited." [PSI:GPS]
is_a: PSI:1000008 ! Ionization Type

[Term]
id: PSI:1000400
name: Plasma Desorption Ionization
def: "The ionization of material in a solid sample by bombarding it with ionic or neutral atoms formed as a result of the fission of a suitable nuclide, typically 252Cf. Synonymous with fission fragment ionization." [PSI:GPS]
is_a: PSI:1000008 ! Ionization Type

[Term]
id: PSI:1000401
name: Pre-Ionization State
def: "An electronic state capable of undergoing auto-Ionization." [PSI:GPS]
is_a: PSI:1000437 ! Ion Reaction Description

[Term]
id: PSI:1000402
name: Secondary Ionization
def: "The process in which ions are ejected from a sample surface as a result of bombardment by a primary beam of atoms or ions." [PSI:GPS]
is_a: PSI:1000008 ! Ionization Type

[Term]
id: PSI:1000403
name: Soft Ionization
def: "The formation of gas-phase ions without extensive fragmentation." [PSI:GPS]
is_a: PSI:1000008 ! Ionization Type

[Term]
id: PSI:1000404
name: Spark Ionization
def: "The formation of ions from a solid material by an intermittent electrical discharge." [PSI:GPS]
is_a: PSI:1000008 ! Ionization Type

[Term]
id: PSI:1000405
name: Surface-Assisted Laser Desorption Ionization
def: "The formation of gas-phase ions from molecules that are deposited on a particular surface substrate that is irradiated with a pulsed laser. See also matrix-assisted laser desorption ionization." [PSI:GPS]
is_a: PSI:1000008 ! Ionization Type

[Term]
id: PSI:1000406
name: Surface Ionization
def: "The ionization of a neutral species when it interacts with a solid surface with an appropriate work function and temperature." [PSI:GPS]
is_a: PSI:1000008 ! Ionization Type

[Term]
id: PSI:1000407
name: Thermal Ionization
def: "The ionization of a neutral species through contact with a high temperature surface." [PSI:GPS]
is_a: PSI:1000008 ! Ionization Type

[Term]
id: PSI:1000408
name: Vertical Ionization
def: "A process in which an electron is removed from or added to a molecule without a change in the positions of the atoms. The resulting ion is typically in an excited vibrational state." [PSI:GPS]
is_a: PSI:1000008 ! Ionization Type

[Term]
id: PSI:1000409
name: Association Reaction
def: "The reaction of an ion with a neutral species in which the reactants combine to form a single ion." [PSI:GPS]
is_a: PSI:1000437 ! Ion Reaction Description

[Term]
id: PSI:1000410
name: Alpha-Cleavage
def: "A homolytic cleavage where the bond fission occurs between at the atom adjacent to the atom at the apparent charge site and an atom removed from the aparent charge site by two bonds." [PSI:GPS]
is_a: PSI:1000437 ! Ion Reaction Description

[Term]
id: PSI:1000411
name: Beta-Cleavage
def: "A homolytic cleavage where the bond fission occurs between at an atom removed from the apparent charge site atom by two bonds and an atom adjacent to that atom and removed from the aparent charge site by three bonds." [PSI:GPS]
is_a: PSI:1000437 ! Ion Reaction Description

[Term]
id: PSI:1000412
name: Buffer Gas
def: "An inert gas used for collisional deactivation of internally excited ions." [PSI:GPS]
relationship: part_of PSI:1000456 ! Precursor Activation Description

[Term]
id: PSI:1000413
name: Charge-Induced Fragmentation
def: "Fragmentation of an odd electron ion in which the cleaved bond is adjacent to the apparent charge site. Synonymous with charge mediated fragmentation." [PSI:GPS]
is_a: PSI:1000437 ! Ion Reaction Description

[Term]
id: PSI:1000414
name: Charge Inversion Reaction
def: "The reaction of an ion with a neutral species in which the charge on the reactant ion is reversed in sign with respect to the product ion." [PSI:GPS]
is_a: PSI:1000437 ! Ion Reaction Description

[Term]
id: PSI:1000415
name: Charge Permutation Reaction
def: "The reaction of an ion with a neutral species with a resulting change in the magnitude or sign of the charge on the reactant ion." [PSI:GPS]
is_a: PSI:1000437 ! Ion Reaction Description

[Term]
id: PSI:1000416
name: Charge Stripping Reaction
def: "The reaction of a positive ion with a neutral species in which the positive charge on the product ion is increased." [PSI:GPS]
is_a: PSI:1000437 ! Ion Reaction Description

[Term]
id: PSI:1000417
name: Charge Transfer Reaction
def: "The reaction of an ion with a neutral species in which some or all of the charge of the reactant ion is transferred to the neutral species." [PSI:GPS]
is_a: PSI:1000437 ! Ion Reaction Description

[Term]
id: PSI:1000418
name: Collisional Excitation
def: "The reaction of an ion with a neutral species in which the translational energy of the collision is converted into internal energy of the ion." [PSI:GPS]
is_a: PSI:1000437 ! Ion Reaction Description

[Term]
id: PSI:1000419
name: Collision Gas
def: "An inert gas used for collisional excitation. The term target gas is not recommended." [PSI:GPS]
relationship: part_of PSI:1000456 ! Precursor Activation Description

[Term]
id: PSI:1000420
name: Heterolytic Cleavage
def: "Fragmentation of an odd electron ion that results from the pair of electrons that form a bond to the atom at the apparent charge site moving to that atom while the charge site moves to the adjacent atom. Fragmentation results in the formation of an even electron ion and a radical. The movement of the pair of electrons is symbolized by a double-barbed arrow. This term is synonymous with heterolysis." [PSI:GPS]
is_a: PSI:1000437 ! Ion Reaction Description

[Term]
id: PSI:1000421
name: High Energy Collision
def: "A collision between an ion and neutral species with translational energy approximately 1000 eV or greater." [PSI:GPS]
is_a: PSI:1000437 ! Ion Reaction Description

[Term]
id: PSI:1000422
name: High-Energy Collision-Induced Dissociation
def: "A collision-induced dissociation process wherein the projectile ion has the translational energy higher than approximately 1000 eV." [PSI:GPS]
relationship: part_of PSI:1000456 ! Precursor Activation Description

[Term]
id: PSI:1000423
name: Homolytic Cleavage
def: "Fragmentation of an odd electron ion that results from one of a pair of electrons that form a bond between two atoms moving to form a pair with the odd electron on the atom at the apparent charge site. Fragmentation results in the formation of an even electron ion and a radical. This reaction involves the movement of a single electron and is symbolized by a single-barbed arrow. Synonymous with Homolysis." [PSI:GPS]
is_a: PSI:1000437 ! Ion Reaction Description

[Term]
id: PSI:1000424
name: Hydrogen/Deuterium Exchange
def: "The exchange of hydrogen with deuterium in solution prior to introduction into a mass spectrometer or by reaction with a deuterated collision gas inside a mass spectrometer." [PSI:GPS]
is_a: PSI:1000437 ! Ion Reaction Description

[Term]
id: PSI:1000425
name: Ion Energy Loss Spectrum
def: "A plot of the relative abundance of a beam or other collection of ions as a function their loss of translational energy in reactions with neutral species." [PSI:GPS]
is_a: PSI:1000442 ! Spectrum

[Term]
id: PSI:1000426
name: Ionizing Collision
def: "The reaction of an ion with a neutral species in which one or more electrons are removed from either the ion or neutral." [PSI:GPS]
is_a: PSI:1000437 ! Ion Reaction Description

[Term]
id: PSI:1000427
name: Ion/Molecule Reaction
def: "The reaction of an ion with a neutral molecule. The term ion-molecule reaction is not recommended because the hyphen suggests a single species that is that is both an ion and a molecule." [PSI:GPS]
is_a: PSI:1000437 ! Ion Reaction Description

[Term]
id: PSI:1000428
name: Ion/Neutral Complex
def: "A transition state that lies between precursor and product ions on the reaction coordinate of an ion fragmentation process." [PSI:GPS]
is_a: PSI:1000437 ! Ion Reaction Description

[Term]
id: PSI:1000429
name: Ion/Neutral Species Reaction
def: "The reaction of an ion with an atom or molecule." [PSI:GPS]
is_a: PSI:1000437 ! Ion Reaction Description

[Term]
id: PSI:1000430
name: Ion/Neutral Species Exchange Reaction
def: "The reaction of an ion with a neutral species to produce a different neutral species as the product." [PSI:GPS]
is_a: PSI:1000437 ! Ion Reaction Description

[Term]
id: PSI:1000431
name: Kinetic Method
def: "An analytical method in which the rate of a reaction or a related quantity is measured and utilized to determine concentrations." [PSI:GPS]
is_a: PSI:1000437 ! Ion Reaction Description

[Term]
id: PSI:1000432
name: Low Energy Collisions
def: "A collision between an ion and neutral species with translational energy approximately 1000 eV or lower." [PSI:GPS]
is_a: PSI:1000437 ! Ion Reaction Description

[Term]
id: PSI:1000433
name: Low-Energy Collision-Induced Dissociation
def: "A collision-induced dissociation process wherein the precursor ion has the translational energy lower than approximately 1000 eV. This process typically requires multiple collisions and the collisional excitation is cumulative." [PSI:GPS]
relationship: part_of PSI:1000456 ! Precursor Activation Description

[Term]
id: PSI:1000434
name: McLafferty Rearrangement
def: "Beta Cleavage with concomitant specific transfer of a y-hydrogen atom in a six-membered transition state in mono-unsaturated systems, irrespective of whether the rearrangement is formulated by a radical or an ionic mechanism, and irrespective of the position of the charge." [PSI:GPS]
is_a: PSI:1000437 ! Ion Reaction Description

[Term]
id: PSI:1000435
name: Photodissociation
def: "A process wherein the reactant ion is dissociated as a result of absorption of one or more photons." [PSI:GPS]
exact_synonym: "Multiphoton Dissociation" []
relationship: part_of PSI:1000456 ! Precursor Activation Description

[Term]
id: PSI:1000436
name: Partial Charge Transfer Reaction
def: "The reaction of an ion with a neutral species in which some but not all of the ion charge is transferred to the neutral." [PSI:GPS]
is_a: PSI:1000437 ! Ion Reaction Description

[Term]
id: PSI:1000437
name: Ion Reaction Description
def: "Chemical transformation involving an ion." [PSI:GPS]
relationship: part_of PSI:0000000 ! mzOntology

[Term]
id: PSI:1000438
name: Superelastic Collision
def: "A collision in which the translational energy of the fast-moving collision partner is increased." [PSI:GPS]
is_a: PSI:1000437 ! Ion Reaction Description

[Term]
id: PSI:1000439
name: Surface-Induced Reaction
def: "A process wherein a reactant ion interacts with a surface to produce either chemically different species or a change in the internal energy of the reactant ion." [PSI:GPS]
is_a: PSI:1000437 ! Ion Reaction Description

[Term]
id: PSI:1000440
name: Unimolecular Dissociation
def: "Fragmentation in which the molecularity is treated as one, irrespective of whether the state results from an metastable ion or from collisional excitation." [PSI:GPS]
is_a: PSI:1000437 ! Ion Reaction Description

[Term]
id: PSI:1000441
name: Scan
def: "TODO: Add definition." [PSI:GPS]
relationship: part_of PSI:0000000 ! mzOntology

[Term]
id: PSI:1000442
name: Spectrum
def: "TODO: Add definition." [PSI:GPS]
relationship: part_of PSI:0000000 ! mzOntology

[Term]
id: PSI:1000443
name: Mass Analyzer
def: "TODO: Add definition." [PSI:GPS]
relationship: part_of PSI:0000000 ! mzOntology

[Term]
id: PSI:1000444
name: m/z Separation Method
def: "TODO: Add definition." [PSI:GPS]
relationship: part_of PSI:0000000 ! mzOntology

[Term]
id: PSI:1000445
name: Sequential m/z Separation Method
def: "TODO: Add definition." [PSI:GPS]
relationship: part_of PSI:0000000 ! mzOntology

[Term]
id: PSI:1000446
name: Fast Ion Bombardment
def: "The ionization of any species by the interaction of a focused beam of ions having a translational energy of several thousand eV with a solid sample." [PSI:GPS]
exact_synonym: "FIB" []
is_a: PSI:1000008 ! Ionization Type

[Term]
id: PSI:1000447
name: LTQ
def: "Finnigan LTQ MS" [PSI:GPS]
is_a: PSI:1000031 ! Model

[Term]
id: PSI:1000448
name: LTQ FT
def: "Finnigan LTQ FT MS" [PSI:GPS]
is_a: PSI:1000031 ! Model

[Term]
id: PSI:1000449
name: LTQ Orbitrap
def: "Finnigan LTQ Orbitrap MS" [PSI:GPS]
is_a: PSI:1000031 ! Model

[Term]
id: PSI:1000450
name: LXQ
def: "Finnigan LXQ MS" [PSI:GPS]
is_a: PSI:1000031 ! Model

[Term]
id: PSI:1000451
name: Analyzer Description
def: "Terms that are used to describe the Analyzer." [PSI:GPS]
relationship: part_of PSI:0000000 ! mzOntology

[Term]
id: PSI:1000452
name: Data Processing Method
def: "Terms used to describe types of data processing." [PSI:GPS]
relationship: part_of PSI:0000000 ! mzOntology

[Term]
id: PSI:1000453
name: Detector Description
def: "Terms that describe the detector." [PSI:GPS]
relationship: part_of PSI:0000000 ! mzOntology

[Term]
id: PSI:1000454
name: Instrument Additional Description
def: "Additional terms to describe the instrument as outlined in the mass spec doc, Appendix 1, section 1.5." [PSI:GPS]
relationship: part_of PSI:0000000 ! mzOntology

[Term]
id: PSI:1000455
name: Ion Selection Description
def: "Terms to decribe the ion." [PSI:GPS]
relationship: part_of PSI:0000000 ! mzOntology

[Term]
id: PSI:1000456
name: Precursor Activation Description
def: "Terms to describe the precursor activation." [PSI:GPS]
relationship: part_of PSI:0000000 ! mzOntology

[Term]
id: PSI:1000457
name: Sample Description
def: "Terms to describe the sample." [PSI:GPS]
relationship: part_of PSI:0000000 ! mzOntology

[Term]
id: PSI:1000458
name: Source Description
def: "Terms to describe the source." [PSI:GPS]
relationship: part_of PSI:0000000 ! mzOntology

[Term]
id: PSI:1000459
name: Spectrum Instrument Description
def: "Terms used to describe the spectrum." [PSI:GPS]
relationship: part_of PSI:0000000 ! mzOntology

[Term]
id: PSI:1000460
name: Unit
def: "Terms to describe units." [PSI:GPS]
relationship: part_of PSI:0000000 ! mzOntology

[Term]
id: PSI:1000461
name: Additional Description
def: "Terms to describe Additional. " [PSI:GPS]
relationship: part_of PSI:0000000 ! mzOntology

[Term]
id: PSI:1000462
name: Ion Optic
def: "Device used in the construction of a spectrometer to focus, contain or otherwise manipulate ions." [PSI:GPS]
relationship: part_of PSI:1000463 ! Instrument

[Term]
id: PSI:1000463
name: Instrument
def: "Device which performs a measurement." [PSI:GPS]
relationship: part_of PSI:0000000 ! mzOntology

[Term]
id: PSI:1000464
name: Mass Unit
def: "A unit of measurement for mass." [PSI:GPS]
is_a: PSI:1000460 ! Unit

[Term]
id: PSI:1000465
name: Polarity Mode
def: "An acquisition mode to which specifies weather polarity is negative, positive or alternating." [PSI:GPS]
relationship: part_of PSI:1000451 ! Analyzer Description
relationship: part_of PSI:1000453 ! Detector Description
relationship: part_of PSI:1000458 ! Source Description

[Term]
id: PSI:1000466
name: Alternating
def: "Alternating." [PSI:GPS]
is_a: PSI:1000465 ! Polarity Mode

[Typedef]
id: part_of
name: part_of
is_transitive: true

